proofs/WOTS_TW.ec
@@ -272,7 +272,7 @@ const trhtype : int.
 
 
 (* -- Notions -- *)
-(*  Number of WOTS-TW instances to consider for D-EF-GCMA notion *)
+(*  Number of WOTS-TW instances to consider for M-EUF-GCMA notion *)
 const d : { int | 1 <= d } as ge1_d.
 
 
@@ -2554,8 +2554,8 @@ module WOTS_TW_ES = {
 
 
 (* -- Adversary classes and oracle interfaces -- *)
-(* Type of oracle given to adversaries in D-EF-GCMA game for WOTS-TW in encompassing structure *)
-module type Oracle_MEFGCMA_WOTSTWES  = {
+(* Type of oracle given to adversaries in M-EUF-GCMA game for WOTS-TW in encompassing structure *)
+module type Oracle_MEUFGCMA_WOTSTWES  = {
   proc init(ss_init : sseed, ps_init : pseed) : unit
   proc query(chad : chadrs, m : msgWOTS) : pkWOTS * sigWOTS
   proc get(i : int) : adrs * msgWOTS * pkWOTS * sigWOTS
@@ -2564,16 +2564,16 @@ module type Oracle_MEFGCMA_WOTSTWES  = {
   proc dist_addresses() : bool
 }.
 
-(* Class of adversaries against D-EF-GCMA game for WOTS-TW in encompassing structure *)
-module type Adv_MEFGCMA_WOTSTWES(O : Oracle_MEFGCMA_WOTSTWES, OC : Oracle_THFC) = {
+(* Class of adversaries against M-EUF-GCMA game for WOTS-TW in encompassing structure *)
+module type Adv_MEUFGCMA_WOTSTWES(O : Oracle_MEUFGCMA_WOTSTWES, OC : Oracle_THFC) = {
   proc choose() : unit { O.query, OC.query }
   proc forge(ps : pseed) : int * msgWOTS * sigWOTS {}
 }.
 
 
 (* -- Notions -- *)
-(* M-EF-GCMA game for WOTS-TW in encompassing structure *) 
-module M_EF_GCMA_WOTSTWES(A : Adv_MEFGCMA_WOTSTWES, O : Oracle_MEFGCMA_WOTSTWES, OC : Oracle_THFC) = {
+(* M-EUF-GCMA game for WOTS-TW in encompassing structure *) 
+module M_EUF_GCMA_WOTSTWES(A : Adv_MEUFGCMA_WOTSTWES, O : Oracle_MEUFGCMA_WOTSTWES, OC : Oracle_THFC) = {
   module A = A(O, OC)
   
   proc main() : bool = {
@@ -2657,8 +2657,8 @@ module M_EF_GCMA_WOTSTWES(A : Adv_MEFGCMA_WOTSTWES, O : Oracle_MEFGCMA_WOTSTWES,
 
 
 (* -- Oracle implementations -- *)
-(* Implementation of signing oracle given to adversary in D-EF-GCMA game for WOTS-TW in encompassing structure *)
-module O_MEFGCMA_WOTSTWES : Oracle_MEFGCMA_WOTSTWES = {
+(* Implementation of signing oracle given to adversary in M-EUF-GCMA game for WOTS-TW in encompassing structure *)
+module O_MEUFGCMA_WOTSTWES : Oracle_MEUFGCMA_WOTSTWES = {
   var ss : sseed
   var ps : pseed
   var qs : (adrs * msgWOTS * pkWOTS * sigWOTS) list
@@ -2706,8 +2706,8 @@ module O_MEFGCMA_WOTSTWES : Oracle_MEFGCMA_WOTSTWES = {
 }.
 
 (* Implementation of oracle given to adversary in the second game of the game sequence. *)
-module O_MEFGCMA_WOTSTWES_NOPRF : Oracle_MEFGCMA_WOTSTWES = {
-  include var O_MEFGCMA_WOTSTWES [-query]
+module O_MEUFGCMA_WOTSTWES_NOPRF : Oracle_MEUFGCMA_WOTSTWES = {
+  include var O_MEUFGCMA_WOTSTWES [-query]
   
   proc query(chad : chadrs, m : msgWOTS) : pkWOTS * sigWOTS = {
     var ad : adrs;
@@ -2753,11 +2753,11 @@ module O_MEFGCMA_WOTSTWES_NOPRF : Oracle_MEFGCMA_WOTSTWES = {
 (* -- Reduction Adversaries -- *)
 (* 
   Reduction adversary that reduces from PRF for prf_sk to distinguishing between
-  Game0_WOTSTWES and MEFGCMA_WOTSTWES without PRF
+  Game0_WOTSTWES and MEUFGCMA_WOTSTWES without PRF
 *)
-module (R_PRF_Game0NOPRFWOTSTWES (A : Adv_MEFGCMA_WOTSTWES) : Adv_PRF) (O : Oracle_PRF) = {
-  module O_R_PRF_Game0NOPRFWOTSTWES : Oracle_MEFGCMA_WOTSTWES = {
-    include var O_MEFGCMA_WOTSTWES [-query]
+module (R_PRF_Game0NOPRFWOTSTWES (A : Adv_MEUFGCMA_WOTSTWES) : Adv_PRF) (O : Oracle_PRF) = {
+  module O_R_PRF_Game0NOPRFWOTSTWES : Oracle_MEUFGCMA_WOTSTWES = {
+    include var O_MEUFGCMA_WOTSTWES [-query]
     
     proc query(chad : chadrs, m : msgWOTS) : pkWOTS * sigWOTS = {
       var ad : adrs;
@@ -2850,7 +2850,7 @@ module (R_PRF_Game0NOPRFWOTSTWES (A : Adv_MEFGCMA_WOTSTWES) : Adv_PRF) (O : Orac
   Game2_WOTSTWES and Game3_WOTSTWES (by, as an intermediate step, reducing to 
   distinguishing between the relevant distributions)
 *)
-module (R_SMDTUDC_Game23WOTSTWES (A : Adv_MEFGCMA_WOTSTWES) : Adv_SMDTUDC) (O : Oracle_SMDTUD) (OC : Oracle_THFC) = {
+module (R_SMDTUDC_Game23WOTSTWES (A : Adv_MEUFGCMA_WOTSTWES) : Adv_SMDTUDC) (O : Oracle_SMDTUD) (OC : Oracle_THFC) = {
   module O_DistRCH = {
     var b : bool
     var ps : pseed
@@ -2909,8 +2909,8 @@ module (R_SMDTUDC_Game23WOTSTWES (A : Adv_MEFGCMA_WOTSTWES) : Adv_SMDTUDC) (O : 
     }
   }
 
-  module O_R_DistRCH_Game23WOTSTW : Oracle_MEFGCMA_WOTSTWES = {
-    include var O_MEFGCMA_WOTSTWES [-query]
+  module O_R_DistRCH_Game23WOTSTW : Oracle_MEUFGCMA_WOTSTWES = {
+    include var O_MEUFGCMA_WOTSTWES [-query]
 
     proc query(chad : chadrs, m : msgWOTS) : pkWOTS * sigWOTS = {
       var ad : adrs;
@@ -3044,9 +3044,9 @@ module (R_SMDTUDC_Game23WOTSTWES (A : Adv_MEFGCMA_WOTSTWES) : Adv_SMDTUDC) (O : 
   Reduction adversary that reduces from SM_DT_TCR_C (for f and thfc) to distinguishing between 
   Game3_WOTSTWES and Game4_WOTSTWES 
 *)
-module (R_SMDTTCRC_Game34WOTSTWES (A : Adv_MEFGCMA_WOTSTWES) : Adv_SMDTTCRC) (O : Oracle_SMDTTCR, OC : Oracle_THFC) = {
-  module O_R_SMDTTCRC_Game34WOTSTWES : Oracle_MEFGCMA_WOTSTWES = {
-    include var O_MEFGCMA_WOTSTWES [-init, query]
+module (R_SMDTTCRC_Game34WOTSTWES (A : Adv_MEUFGCMA_WOTSTWES) : Adv_SMDTTCRC) (O : Oracle_SMDTTCR, OC : Oracle_THFC) = {
+  module O_R_SMDTTCRC_Game34WOTSTWES : Oracle_MEUFGCMA_WOTSTWES = {
+    include var O_MEUFGCMA_WOTSTWES [-init, query]
     var xll : dgstblock list list
     
     proc init(ss_init : sseed, ps_init : pseed) = {
@@ -3154,9 +3154,9 @@ module (R_SMDTTCRC_Game34WOTSTWES (A : Adv_MEFGCMA_WOTSTWES) : Adv_SMDTTCRC) (O 
 }.
 
 (* Reduction adversary that reduces from SM_DT_PRE_C (for f and thfc) to Game4_WOTSTWES *)
-module (R_SMDTPREC_Game4WOTSTWES (A : Adv_MEFGCMA_WOTSTWES) : Adv_SMDTPREC) (O : Oracle_SMDTPRE, OC : Oracle_THFC) = {
-  module O_R_SMDTPREC_Game4WOTSTWES : Oracle_MEFGCMA_WOTSTWES = {
-    include var O_MEFGCMA_WOTSTWES [-query, init]
+module (R_SMDTPREC_Game4WOTSTWES (A : Adv_MEUFGCMA_WOTSTWES) : Adv_SMDTPREC) (O : Oracle_SMDTPRE, OC : Oracle_THFC) = {
+  module O_R_SMDTPREC_Game4WOTSTWES : Oracle_MEUFGCMA_WOTSTWES = {
+    include var O_MEUFGCMA_WOTSTWES [-query, init]
     var adl : adrs list
     
     proc init(ss_init : sseed, ps_init : pseed) = {
@@ -3257,8 +3257,8 @@ module (R_SMDTPREC_Game4WOTSTWES (A : Adv_MEFGCMA_WOTSTWES) : Adv_SMDTPREC) (O :
 }.
 
 
-(* -- Proof of M-EF-GCMA for WOTS-TW (in an encompassing structure) -- *)
-section Proof_M_EF_GCMA_WOTSTWES.
+(* -- Proof of M-EUF-GCMA for WOTS-TW (in an encompassing structure) -- *)
+section Proof_M_EUF_GCMA_WOTSTWES.
 (* - (Auxiliary) Imports - *)
 (* 
   Import necessary definitions/properties to reason about programs sampling from
@@ -3284,9 +3284,9 @@ local module type Adv_DistRCH(O : Oracle_DistRCH, OC : Oracle_THFC) = {
 
 
 (* - Module declarations - *)
-(* Adversary against M-EF-GCMA of WOTW-TW (in an encompassing structure) *)
-declare module A <: Adv_MEFGCMA_WOTSTWES {
-  -O_MEFGCMA_WOTSTWES, -O_PRF_Default, -O_SMDTUD_Default, -O_SMDTTCR_Default, -O_SMDTPRE_Default, -O_THFC_Default,
+(* Adversary against M-EUF-GCMA of WOTW-TW (in an encompassing structure) *)
+declare module A <: Adv_MEUFGCMA_WOTSTWES {
+  -O_MEUFGCMA_WOTSTWES, -O_PRF_Default, -O_SMDTUD_Default, -O_SMDTTCR_Default, -O_SMDTPRE_Default, -O_THFC_Default,
   -R_SMDTUDC_Game23WOTSTWES, -R_SMDTTCRC_Game34WOTSTWES, -R_SMDTPREC_Game4WOTSTWES, -R_PRF_Game0NOPRFWOTSTWES
 }.
 
@@ -3294,18 +3294,18 @@ declare module A <: Adv_MEFGCMA_WOTSTWES {
   The adversary's choose procedure always terminates if the oracle procedures it can 
   call during its execution terminate 
 *)
-declare axiom A_choose_ll (O <: Oracle_MEFGCMA_WOTSTWES {-A} ) (OC <: Oracle_THFC {-A} ) :
+declare axiom A_choose_ll (O <: Oracle_MEUFGCMA_WOTSTWES {-A} ) (OC <: Oracle_THFC {-A} ) :
   islossless O.query => islossless OC.query => islossless A(O, OC).choose.
 
 (* The adversary's forge procedure always terminates *)
-declare axiom A_forge_ll (O <: Oracle_MEFGCMA_WOTSTWES {-A} ) (OC <: Oracle_THFC {-A} ) :
+declare axiom A_forge_ll (O <: Oracle_MEUFGCMA_WOTSTWES {-A} ) (OC <: Oracle_THFC {-A} ) :
   islossless A(O, OC).forge.
 
 
 (* - Oracle implementations - *)
 (* Implementation of oracle given to adversary in Game0_WOTSTWES. *)
-local module O_Game0_WOTSTWES : Oracle_MEFGCMA_WOTSTWES = {
-  include var O_MEFGCMA_WOTSTWES [-query]
+local module O_Game0_WOTSTWES : Oracle_MEUFGCMA_WOTSTWES = {
+  include var O_MEUFGCMA_WOTSTWES [-query]
   
   proc query(chad : chadrs, m : msgWOTS) : pkWOTS * sigWOTS = {
     var ad : adrs;
@@ -3355,8 +3355,8 @@ local module O_Game0_WOTSTWES : Oracle_MEFGCMA_WOTSTWES = {
   Implementation of oracle given to adversary in Game2_WOTSTWES.
   Swaps signing and public key generation.
 *)
-local module O_Game2_WOTSTWES : Oracle_MEFGCMA_WOTSTWES = {
-  include var O_MEFGCMA_WOTSTWES [-query]
+local module O_Game2_WOTSTWES : Oracle_MEUFGCMA_WOTSTWES = {
+  include var O_MEUFGCMA_WOTSTWES [-query]
   
   proc query(chad : chadrs, m : msgWOTS) : pkWOTS * sigWOTS = {
     var ad : adrs;
@@ -3404,8 +3404,8 @@ local module O_Game2_WOTSTWES : Oracle_MEFGCMA_WOTSTWES = {
   to get signature (instead of chaining from 0 to this index). Afterward, public key
   is computed by finishing the chains of the signature.
 *)
-local module O_Game34_WOTSTWES : Oracle_MEFGCMA_WOTSTWES = {
-  include var O_MEFGCMA_WOTSTWES [-query]
+local module O_Game34_WOTSTWES : Oracle_MEUFGCMA_WOTSTWES = {
+  include var O_MEUFGCMA_WOTSTWES [-query]
   
   proc query(chad : chadrs, m : msgWOTS) : pkWOTS * sigWOTS = {
     var ad : adrs;
@@ -3493,11 +3493,11 @@ local module O_DistRCH : Oracle_DistRCH = {
 }.
 
 (* 
-  Auxiliary implementations for O_MEFGCMA_WOTSTWES_NOPRF, used to obtain the desired form
+  Auxiliary implementations for O_MEUFGCMA_WOTSTWES_NOPRF, used to obtain the desired form
   for the proof of the PRF reduction 
 *)  
-local module O_MEFGCMA_WOTSTWES_NOPRF_SampleSample : Oracle_MEFGCMA_WOTSTWES = {
-  include var O_MEFGCMA_WOTSTWES [-query]
+local module O_MEUFGCMA_WOTSTWES_NOPRF_SampleSample : Oracle_MEUFGCMA_WOTSTWES = {
+  include var O_MEUFGCMA_WOTSTWES [-query]
   
   proc query(chad : chadrs, m : msgWOTS) : pkWOTS * sigWOTS = {
     var ad : adrs;
@@ -3539,8 +3539,8 @@ local module O_MEFGCMA_WOTSTWES_NOPRF_SampleSample : Oracle_MEFGCMA_WOTSTWES = {
   }
 }.
 
-local module O_MEFGCMA_WOTSTWES_NOPRF_LoopSnocSample : Oracle_MEFGCMA_WOTSTWES = {
-  include var O_MEFGCMA_WOTSTWES [-query]
+local module O_MEUFGCMA_WOTSTWES_NOPRF_LoopSnocSample : Oracle_MEUFGCMA_WOTSTWES = {
+  include var O_MEUFGCMA_WOTSTWES [-query]
   
   proc query(chad : chadrs, m : msgWOTS) : pkWOTS * sigWOTS = {
     var ad : adrs;
@@ -3582,8 +3582,8 @@ local module O_MEFGCMA_WOTSTWES_NOPRF_LoopSnocSample : Oracle_MEFGCMA_WOTSTWES =
   }
 }.
 
-local module O_MEFGCMA_WOTSTWES_NOPRF_Alt : Oracle_MEFGCMA_WOTSTWES = {
-  include var O_MEFGCMA_WOTSTWES [-query]
+local module O_MEUFGCMA_WOTSTWES_NOPRF_Alt : Oracle_MEUFGCMA_WOTSTWES = {
+  include var O_MEUFGCMA_WOTSTWES [-query]
   
   proc query(chad : chadrs, m : msgWOTS) : pkWOTS * sigWOTS = {
     var ad : adrs;
@@ -3629,30 +3629,30 @@ local module O_MEFGCMA_WOTSTWES_NOPRF_Alt : Oracle_MEFGCMA_WOTSTWES = {
   }
 }.
 
-(* Equivalences between original and auxiliary implementations of O_MEFGCMA_WOTSTWES_NOPRF *)
-local equiv O_MEFGCMA_WOTSTWES_NOPRF_Orig_SampleSample : 
-  O_MEFGCMA_WOTSTWES_NOPRF.query ~ O_MEFGCMA_WOTSTWES_NOPRF_SampleSample.query : 
-    ={O_MEFGCMA_WOTSTWES.ps, O_MEFGCMA_WOTSTWES.qs, chad, m} ==> ={O_MEFGCMA_WOTSTWES.ps, O_MEFGCMA_WOTSTWES.qs, res}.
+(* Equivalences between original and auxiliary implementations of O_MEUFGCMA_WOTSTWES_NOPRF *)
+local equiv O_MEUFGCMA_WOTSTWES_NOPRF_Orig_SampleSample : 
+  O_MEUFGCMA_WOTSTWES_NOPRF.query ~ O_MEUFGCMA_WOTSTWES_NOPRF_SampleSample.query : 
+    ={O_MEUFGCMA_WOTSTWES.ps, O_MEUFGCMA_WOTSTWES.qs, chad, m} ==> ={O_MEUFGCMA_WOTSTWES.ps, O_MEUFGCMA_WOTSTWES.qs, res}.
 proof.
 proc; inline *.
 by sim; auto.
 qed.
 
-local equiv O_MEFGCMA_WOTSTWES_NOPRF_SampleSample_LoopSnocSample : 
-  O_MEFGCMA_WOTSTWES_NOPRF_SampleSample.query ~ O_MEFGCMA_WOTSTWES_NOPRF_LoopSnocSample.query : 
-    ={O_MEFGCMA_WOTSTWES.ps, O_MEFGCMA_WOTSTWES.qs, chad, m} ==> ={O_MEFGCMA_WOTSTWES.ps, O_MEFGCMA_WOTSTWES.qs, res}.
+local equiv O_MEUFGCMA_WOTSTWES_NOPRF_SampleSample_LoopSnocSample : 
+  O_MEUFGCMA_WOTSTWES_NOPRF_SampleSample.query ~ O_MEUFGCMA_WOTSTWES_NOPRF_LoopSnocSample.query : 
+    ={O_MEUFGCMA_WOTSTWES.ps, O_MEUFGCMA_WOTSTWES.qs, chad, m} ==> ={O_MEUFGCMA_WOTSTWES.ps, O_MEUFGCMA_WOTSTWES.qs, res}.
 proof.
 proc.
 seq 2 2 : (#pre /\ ={ad, sk}) => /=; last by sim.
 by sp; call Sample_LoopSnoc_eq; skip.
 qed.
 
-local equiv O_MEFGCMA_WOTSTWES_NOPRF_LoopSnocSample_Alt : 
-  O_MEFGCMA_WOTSTWES_NOPRF_LoopSnocSample.query ~ O_MEFGCMA_WOTSTWES_NOPRF_Alt.query : 
-    ={O_MEFGCMA_WOTSTWES.ps, O_MEFGCMA_WOTSTWES.qs, chad, m} ==> ={O_MEFGCMA_WOTSTWES.ps, O_MEFGCMA_WOTSTWES.qs, res}.
+local equiv O_MEUFGCMA_WOTSTWES_NOPRF_LoopSnocSample_Alt : 
+  O_MEUFGCMA_WOTSTWES_NOPRF_LoopSnocSample.query ~ O_MEUFGCMA_WOTSTWES_NOPRF_Alt.query : 
+    ={O_MEUFGCMA_WOTSTWES.ps, O_MEUFGCMA_WOTSTWES.qs, chad, m} ==> ={O_MEUFGCMA_WOTSTWES.ps, O_MEUFGCMA_WOTSTWES.qs, res}.
 proof.
 proc; inline *.
-seq 5 3 : (={O_MEFGCMA_WOTSTWES.ps, O_MEFGCMA_WOTSTWES.qs, ad, m} /\ l{1} = sk{2}); last by sim => /#.
+seq 5 3 : (={O_MEUFGCMA_WOTSTWES.ps, O_MEUFGCMA_WOTSTWES.qs, ad, m} /\ l{1} = sk{2}); last by sim => /#.
 while (   #post
        /\ n{1} = len
        /\ i{1} = size sk{2} 
@@ -3660,27 +3660,27 @@ while (   #post
 by wp; rnd; skip => />; smt(size_rcons cats1).
 qed.
 
-local equiv O_MEFGCMA_WOTSTWES_NOPRF_Orig_Alt : 
-  O_MEFGCMA_WOTSTWES_NOPRF.query ~ O_MEFGCMA_WOTSTWES_NOPRF_Alt.query : 
-    ={O_MEFGCMA_WOTSTWES.ps, O_MEFGCMA_WOTSTWES.qs, chad, m} ==> ={O_MEFGCMA_WOTSTWES.ps, O_MEFGCMA_WOTSTWES.qs, res}.
+local equiv O_MEUFGCMA_WOTSTWES_NOPRF_Orig_Alt : 
+  O_MEUFGCMA_WOTSTWES_NOPRF.query ~ O_MEUFGCMA_WOTSTWES_NOPRF_Alt.query : 
+    ={O_MEUFGCMA_WOTSTWES.ps, O_MEUFGCMA_WOTSTWES.qs, chad, m} ==> ={O_MEUFGCMA_WOTSTWES.ps, O_MEUFGCMA_WOTSTWES.qs, res}.
 proof.
-transitivity O_MEFGCMA_WOTSTWES_NOPRF_SampleSample.query 
-             (={O_MEFGCMA_WOTSTWES.ps, O_MEFGCMA_WOTSTWES.qs, chad, m} ==> ={O_MEFGCMA_WOTSTWES.ps, O_MEFGCMA_WOTSTWES.qs, res}) 
-             (={O_MEFGCMA_WOTSTWES.ps, O_MEFGCMA_WOTSTWES.qs, chad, m} ==> ={O_MEFGCMA_WOTSTWES.ps, O_MEFGCMA_WOTSTWES.qs, res}) => [/# | // | |].
-+ by apply O_MEFGCMA_WOTSTWES_NOPRF_Orig_SampleSample.
-transitivity O_MEFGCMA_WOTSTWES_NOPRF_LoopSnocSample.query 
-             (={O_MEFGCMA_WOTSTWES.ps, O_MEFGCMA_WOTSTWES.qs, chad, m} ==> ={O_MEFGCMA_WOTSTWES.ps, O_MEFGCMA_WOTSTWES.qs, res}) 
-             (={O_MEFGCMA_WOTSTWES.ps, O_MEFGCMA_WOTSTWES.qs, chad, m} ==> ={O_MEFGCMA_WOTSTWES.ps, O_MEFGCMA_WOTSTWES.qs, res}) => [/# | // | |].
-+ by apply O_MEFGCMA_WOTSTWES_NOPRF_SampleSample_LoopSnocSample.
-by apply O_MEFGCMA_WOTSTWES_NOPRF_LoopSnocSample_Alt.
+transitivity O_MEUFGCMA_WOTSTWES_NOPRF_SampleSample.query 
+             (={O_MEUFGCMA_WOTSTWES.ps, O_MEUFGCMA_WOTSTWES.qs, chad, m} ==> ={O_MEUFGCMA_WOTSTWES.ps, O_MEUFGCMA_WOTSTWES.qs, res}) 
+             (={O_MEUFGCMA_WOTSTWES.ps, O_MEUFGCMA_WOTSTWES.qs, chad, m} ==> ={O_MEUFGCMA_WOTSTWES.ps, O_MEUFGCMA_WOTSTWES.qs, res}) => [/# | // | |].
++ by apply O_MEUFGCMA_WOTSTWES_NOPRF_Orig_SampleSample.
+transitivity O_MEUFGCMA_WOTSTWES_NOPRF_LoopSnocSample.query 
+             (={O_MEUFGCMA_WOTSTWES.ps, O_MEUFGCMA_WOTSTWES.qs, chad, m} ==> ={O_MEUFGCMA_WOTSTWES.ps, O_MEUFGCMA_WOTSTWES.qs, res}) 
+             (={O_MEUFGCMA_WOTSTWES.ps, O_MEUFGCMA_WOTSTWES.qs, chad, m} ==> ={O_MEUFGCMA_WOTSTWES.ps, O_MEUFGCMA_WOTSTWES.qs, res}) => [/# | // | |].
++ by apply O_MEUFGCMA_WOTSTWES_NOPRF_SampleSample_LoopSnocSample.
+by apply O_MEUFGCMA_WOTSTWES_NOPRF_LoopSnocSample_Alt.
 qed.
 
 (* 
   Auxiliary implementations for O_Game34_WOTSTWES, used to obtain the desired form
   for the proof of the SM_DT_PRE_C reduction 
 *)  
-local module O_Game34_WOTSTWES_SampleSample : Oracle_MEFGCMA_WOTSTWES = {
-  include var O_MEFGCMA_WOTSTWES [-query]
+local module O_Game34_WOTSTWES_SampleSample : Oracle_MEUFGCMA_WOTSTWES = {
+  include var O_MEUFGCMA_WOTSTWES [-query]
   
   proc query(chad : chadrs, m : msgWOTS) : pkWOTS * sigWOTS = {
     var ad : adrs;
@@ -3729,8 +3729,8 @@ local module O_Game34_WOTSTWES_SampleSample : Oracle_MEFGCMA_WOTSTWES = {
   }
 }.
 
-local module O_Game34_WOTSTWES_LoopSnocSample : Oracle_MEFGCMA_WOTSTWES = {
-  include var O_MEFGCMA_WOTSTWES [-query]
+local module O_Game34_WOTSTWES_LoopSnocSample : Oracle_MEUFGCMA_WOTSTWES = {
+  include var O_MEUFGCMA_WOTSTWES [-query]
   
   proc query(chad : chadrs, m : msgWOTS) : pkWOTS * sigWOTS = {
     var ad : adrs;
@@ -3782,8 +3782,8 @@ local module O_Game34_WOTSTWES_LoopSnocSample : Oracle_MEFGCMA_WOTSTWES = {
   }
 }.
 
-local module O_Game34_WOTSTWES_LoopSnocSampleAlt : Oracle_MEFGCMA_WOTSTWES = {
-  include var O_MEFGCMA_WOTSTWES [-query]
+local module O_Game34_WOTSTWES_LoopSnocSampleAlt : Oracle_MEUFGCMA_WOTSTWES = {
+  include var O_MEUFGCMA_WOTSTWES [-query]
   
   proc query(chad : chadrs, m : msgWOTS) : pkWOTS * sigWOTS = {
     var ad : adrs;
@@ -3836,8 +3836,8 @@ local module O_Game34_WOTSTWES_LoopSnocSampleAlt : Oracle_MEFGCMA_WOTSTWES = {
   }
 }.
 
-local module O_Game34_WOTSTWES_Alt : Oracle_MEFGCMA_WOTSTWES = {
-  include var O_MEFGCMA_WOTSTWES [-query]
+local module O_Game34_WOTSTWES_Alt : Oracle_MEUFGCMA_WOTSTWES = {
+  include var O_MEUFGCMA_WOTSTWES [-query]
   
   proc query(chad : chadrs, m : msgWOTS) : pkWOTS * sigWOTS = {
     var ad : adrs;
@@ -3889,7 +3889,7 @@ local module O_Game34_WOTSTWES_Alt : Oracle_MEFGCMA_WOTSTWES = {
 (* Equivalences between original and auxiliary implementations of O_Game34_WOTSTWES *)
 local equiv O_Game34_WOTSTWES_Orig_SampleSample : 
   O_Game34_WOTSTWES.query ~ O_Game34_WOTSTWES_SampleSample.query : 
-    ={glob O_MEFGCMA_WOTSTWES, chad, m} ==> ={glob O_MEFGCMA_WOTSTWES, res}.
+    ={glob O_MEUFGCMA_WOTSTWES, chad, m} ==> ={glob O_MEUFGCMA_WOTSTWES, res}.
 proof.
 proc; inline *.
 by sim; auto.
@@ -3897,13 +3897,13 @@ qed.
 
 local equiv O_Game34_WOTSTWES_SampleSample_LoopSnocSample : 
   O_Game34_WOTSTWES_SampleSample.query ~ O_Game34_WOTSTWES_LoopSnocSample.query : 
-    ={glob O_MEFGCMA_WOTSTWES, chad, m} ==> ={glob O_MEFGCMA_WOTSTWES, res}.
+    ={glob O_MEUFGCMA_WOTSTWES, chad, m} ==> ={glob O_MEUFGCMA_WOTSTWES, res}.
 proof.
 proc.
 seq 2 2 : (#pre /\ ={ad, sk}) => /=.
 + by sp; call Sample_LoopSnoc_eq; skip.
 sp; sim.
-while (   ={O_MEFGCMA_WOTSTWES.ps, ad, m, sk, sig, em}
+while (   ={O_MEUFGCMA_WOTSTWES.ps, ad, m, sk, sig, em}
        /\ size sig{1} = i{2}
        /\ 0 <= i{2} <= len
        /\ 0 <= size sig{1} <= len).
@@ -3913,12 +3913,12 @@ qed.
 
 local equiv O_Game34_WOTSTWES_LoopSnocSample_LoopSnocSampleAlt : 
   O_Game34_WOTSTWES_LoopSnocSample.query ~ O_Game34_WOTSTWES_LoopSnocSampleAlt.query : 
-    ={glob O_MEFGCMA_WOTSTWES, chad, m} ==> ={glob O_MEFGCMA_WOTSTWES, res}.
+    ={glob O_MEUFGCMA_WOTSTWES, chad, m} ==> ={glob O_MEUFGCMA_WOTSTWES, res}.
 proof.
 proc; inline *.
 seq 9 5 : (#pre /\ ={ad, sk, em, sig} /\  i{1} = 0 /\ sig{1} = [] /\ sig{2} = []) => /=.
 + sp; wp => /=.
-  while (   ={O_MEFGCMA_WOTSTWES.ps, ad, m}
+  while (   ={O_MEUFGCMA_WOTSTWES.ps, ad, m}
          /\ n{1} = len
          /\ l{1} = sk{2}
          /\ i0{1} = size sk{2}
@@ -3927,7 +3927,7 @@ seq 9 5 : (#pre /\ ={ad, sk, em, sig} /\  i{1} = 0 /\ sig{1} = [] /\ sig{2} = []
   - by auto => />; smt(cats1 size_rcons).
   by auto => />; smt(ge2_len).
 sim => /=.
-while (   ={O_MEFGCMA_WOTSTWES.ps, ad, m, sk, em, sig}
+while (   ={O_MEUFGCMA_WOTSTWES.ps, ad, m, sk, em, sig}
        /\ i{1} = size sig{2}
        /\ 0 <= i{1} <= len
        /\ 0 <= size sig{2} <= len).
@@ -3937,7 +3937,7 @@ qed.
 
 local equiv O_Game34_WOTSTWES_LoopSnocSampleAlt_Alt : 
   O_Game34_WOTSTWES_LoopSnocSampleAlt.query ~ O_Game34_WOTSTWES_Alt.query : 
-    ={glob O_MEFGCMA_WOTSTWES, chad, m} ==> ={glob O_MEFGCMA_WOTSTWES, res}.
+    ={glob O_MEUFGCMA_WOTSTWES, chad, m} ==> ={glob O_MEUFGCMA_WOTSTWES, res}.
 proof.
 proc; inline *.
 seq 5 5 : (   #pre 
@@ -3946,17 +3946,17 @@ seq 5 5 : (   #pre
            /\ (forall (i : int), 0 <= i < len =>
                  nth witness sig{2} i =
                  if BaseW.val em{2}.[i] <> 0
-                 then cf O_MEFGCMA_WOTSTWES.ps{2} (set_chthidx ad{2} i) (BaseW.val em{2}.[i] - 1) 1 (val (nth witness sk{2} i))
+                 then cf O_MEUFGCMA_WOTSTWES.ps{2} (set_chthidx ad{2} i) (BaseW.val em{2}.[i] - 1) 1 (val (nth witness sk{2} i))
                  else nth witness sk{2} i)
            /\ size sig{2} = len) => /=.
 + swap{1} [4..5] -1; swap{2} 3 -1; sp; wp => /=.
-  while (   ={O_MEFGCMA_WOTSTWES.ps, ad, m, sk, em}
+  while (   ={O_MEUFGCMA_WOTSTWES.ps, ad, m, sk, em}
          /\ is_chtype ad{1}
          /\ sig{1} = [] 
          /\ (forall (i : int), 0 <= i < size sig{2} =>
                nth witness sig{2} i =
                if BaseW.val em{2}.[i] <> 0
-               then cf O_MEFGCMA_WOTSTWES.ps{2} (set_chthidx ad{2} i) (BaseW.val em{2}.[i] - 1) 1 (val (nth witness sk{2} i))
+               then cf O_MEUFGCMA_WOTSTWES.ps{2} (set_chthidx ad{2} i) (BaseW.val em{2}.[i] - 1) 1 (val (nth witness sk{2} i))
                else nth witness sk{2} i)
          /\ size sk{1} = size sig{2}
          /\ 0 <= size sk{1} <= len
@@ -3970,12 +3970,12 @@ seq 5 5 : (   #pre
     by rewrite (: i = size sig{1}) 1:/# neq0_em.
   by skip => />; smt(ge2_len ChainingAddress.valP).
 sim => /=.
-while{1} (   ={O_MEFGCMA_WOTSTWES.ps, ad, m, sk, em}
+while{1} (   ={O_MEUFGCMA_WOTSTWES.ps, ad, m, sk, em}
           /\ (forall (i : int),
                0 <= i && i < len =>
                nth witness sig{2} i =
                if BaseW.val em{2}.[i] <> 0
-               then cf O_MEFGCMA_WOTSTWES.ps{2} (set_chthidx ad{2} i) (BaseW.val em{2}.[i] - 1) 1 (val (nth witness sk{2} i))
+               then cf O_MEUFGCMA_WOTSTWES.ps{2} (set_chthidx ad{2} i) (BaseW.val em{2}.[i] - 1) 1 (val (nth witness sk{2} i))
                else nth witness sk{2} i)
           /\ (forall (i : int), 0 <= i < size sig{1} =>
                 nth witness sig{1} i = nth witness sig{2} i)
@@ -3992,19 +3992,19 @@ qed.
 
 local equiv O_Game34_WOTSTWES_Orig_Alt : 
   O_Game34_WOTSTWES.query ~ O_Game34_WOTSTWES_Alt.query : 
-    ={glob O_MEFGCMA_WOTSTWES, chad, m} ==> ={glob O_MEFGCMA_WOTSTWES, res}.
+    ={glob O_MEUFGCMA_WOTSTWES, chad, m} ==> ={glob O_MEUFGCMA_WOTSTWES, res}.
 proof.
 transitivity O_Game34_WOTSTWES_SampleSample.query 
-             (={glob O_MEFGCMA_WOTSTWES, chad, m} ==> ={glob O_MEFGCMA_WOTSTWES, res}) 
-             (={glob O_MEFGCMA_WOTSTWES, chad, m} ==> ={glob O_MEFGCMA_WOTSTWES, res}) => [/# | // | |].
+             (={glob O_MEUFGCMA_WOTSTWES, chad, m} ==> ={glob O_MEUFGCMA_WOTSTWES, res}) 
+             (={glob O_MEUFGCMA_WOTSTWES, chad, m} ==> ={glob O_MEUFGCMA_WOTSTWES, res}) => [/# | // | |].
 + by apply O_Game34_WOTSTWES_Orig_SampleSample.
 transitivity O_Game34_WOTSTWES_LoopSnocSample.query 
-             (={glob O_MEFGCMA_WOTSTWES, chad, m} ==> ={glob O_MEFGCMA_WOTSTWES, res}) 
-             (={glob O_MEFGCMA_WOTSTWES, chad, m} ==> ={glob O_MEFGCMA_WOTSTWES, res}) => [/# | // | |].
+             (={glob O_MEUFGCMA_WOTSTWES, chad, m} ==> ={glob O_MEUFGCMA_WOTSTWES, res}) 
+             (={glob O_MEUFGCMA_WOTSTWES, chad, m} ==> ={glob O_MEUFGCMA_WOTSTWES, res}) => [/# | // | |].
 + by apply O_Game34_WOTSTWES_SampleSample_LoopSnocSample.
 transitivity O_Game34_WOTSTWES_LoopSnocSampleAlt.query 
-             (={glob O_MEFGCMA_WOTSTWES, chad, m} ==> ={glob O_MEFGCMA_WOTSTWES, res}) 
-             (={glob O_MEFGCMA_WOTSTWES, chad, m} ==> ={glob O_MEFGCMA_WOTSTWES, res}) => [/# | // | |].
+             (={glob O_MEUFGCMA_WOTSTWES, chad, m} ==> ={glob O_MEUFGCMA_WOTSTWES, res}) 
+             (={glob O_MEUFGCMA_WOTSTWES, chad, m} ==> ={glob O_MEUFGCMA_WOTSTWES, res}) => [/# | // | |].
 + by apply O_Game34_WOTSTWES_LoopSnocSample_LoopSnocSampleAlt.
 by apply O_Game34_WOTSTWES_LoopSnocSampleAlt_Alt.
 qed.
@@ -4013,31 +4013,31 @@ qed.
 (* - Games in game sequence - *)
 (* 
   Game0_WOTSTWES; first game in game sequence.
-  Identical to M_EF_GCMA_WOTSTWES, only differing in the query procedure of the 
-  provided Oracle_MEFGCMA_WOTSTWES (see above for the different oracle implementations). 
+  Identical to M_EUF_GCMA_WOTSTWES, only differing in the query procedure of the 
+  provided Oracle_MEUFGCMA_WOTSTWES (see above for the different oracle implementations). 
 *)
 local module Game0_WOTSTWES = {
-  include M_EF_GCMA_WOTSTWES(A, O_Game0_WOTSTWES, O_THFC_Default)
+  include M_EUF_GCMA_WOTSTWES(A, O_Game0_WOTSTWES, O_THFC_Default)
 }.
  
 (* 
   Game2_WOTSTWES; third game in game sequence.
-  Identical to M_EF_GCMA_WOTSTWES, only differing in the 
-  query procedure of the provided Oracle_MEFGCMA_WOTSTWES (see above for the 
+  Identical to M_EUF_GCMA_WOTSTWES, only differing in the 
+  query procedure of the provided Oracle_MEUFGCMA_WOTSTWES (see above for the 
   different oracle implementations).
 *)
 local module Game2_WOTSTWES = {
-  include M_EF_GCMA_WOTSTWES(A, O_Game2_WOTSTWES, O_THFC_Default)
+  include M_EUF_GCMA_WOTSTWES(A, O_Game2_WOTSTWES, O_THFC_Default)
 }.
 
 (* 
   Game3_WOTSTWES; fourth game in game sequence.
-  Identical to M_EF_GCMA_WOTSTWES (and hence to Game2_WOTSTWES), only differing in the 
-  query procedure of the provided Oracle_MEFGCMA_WOTSTWES (see above for the 
+  Identical to M_EUF_GCMA_WOTSTWES (and hence to Game2_WOTSTWES), only differing in the 
+  query procedure of the provided Oracle_MEUFGCMA_WOTSTWES (see above for the 
   different oracle implementations).
 *)
 local module Game3_WOTSTWES = {
-  include M_EF_GCMA_WOTSTWES(A, O_Game34_WOTSTWES, O_THFC_Default)
+  include M_EUF_GCMA_WOTSTWES(A, O_Game34_WOTSTWES, O_THFC_Default)
 }.
 
 (* 
@@ -4201,10 +4201,10 @@ local equiv Game4_WOTSTWES_Orig_Alt :
 proof.
 proc; inline *.
 seq 1 1 : (#pre /\ ={ps}); first by rnd.
-seq 9 9 : (={glob A, glob O_MEFGCMA_WOTSTWES, glob O_THFC_Default, ps}); last by sim.
+seq 9 9 : (={glob A, glob O_MEUFGCMA_WOTSTWES, glob O_THFC_Default, ps}); last by sim.
 sp => /=.
-call (: ={glob O_MEFGCMA_WOTSTWES, glob O_THFC_Default}); last by auto.
-+ conseq (: ={glob O_MEFGCMA_WOTSTWES, chad, m} ==> ={glob O_MEFGCMA_WOTSTWES, res}) => //.
+call (: ={glob O_MEUFGCMA_WOTSTWES, glob O_THFC_Default}); last by auto.
++ conseq (: ={glob O_MEUFGCMA_WOTSTWES, chad, m} ==> ={glob O_MEUFGCMA_WOTSTWES, res}) => //.
   by apply O_Game34_WOTSTWES_Orig_Alt.
 by sim.
 qed.
@@ -4216,8 +4216,8 @@ qed.
   to distinguishing between Game2_WOTSTWES and Game3_WOTSTWES.
 *)
 local module (R_DistRCH_Game23WOTSTW : Adv_DistRCH) (O : Oracle_DistRCH, OC : Oracle_THFC) = {
-  module O_R_DistRCH_Game23WOTSTW : Oracle_MEFGCMA_WOTSTWES = {
-    include var O_MEFGCMA_WOTSTWES [-query]
+  module O_R_DistRCH_Game23WOTSTW : Oracle_MEUFGCMA_WOTSTWES = {
+    include var O_MEUFGCMA_WOTSTWES [-query]
 
     proc query(chad : chadrs, m : msgWOTS) : pkWOTS * sigWOTS = {
       var ad : adrs;
@@ -4712,8 +4712,8 @@ local equiv DistRCHi_Orig_SampleSample :
     ={glob A, i} ==> ={res}.
 proof.
 proc; inline *.
-seq 18 18 : (={glob A, glob O_MEFGCMA_WOTSTWES, R_DistRCH_Game23WOTSTW.O_R_DistRCH_Game23WOTSTW_THFC.adl, ps}); last by sim.
-call (:   ={glob O_THFC_Default, glob O_MEFGCMA_WOTSTWES, glob O_DistRCH, R_DistRCH_Game23WOTSTW.O_R_DistRCH_Game23WOTSTW_THFC.adl} 
+seq 18 18 : (={glob A, glob O_MEUFGCMA_WOTSTWES, R_DistRCH_Game23WOTSTW.O_R_DistRCH_Game23WOTSTW_THFC.adl, ps}); last by sim.
+call (:   ={glob O_THFC_Default, glob O_MEUFGCMA_WOTSTWES, glob O_DistRCH, R_DistRCH_Game23WOTSTW.O_R_DistRCH_Game23WOTSTW_THFC.adl} 
        /\ DistRCHi.O_DistRCHi.i{1} = DistRCHi_SampleSample.O_DistRCHi.i{2}) => //=.
 + proc; inline *.
   by sim; rnd; wp; skip.
@@ -4726,8 +4726,8 @@ local equiv DistRCHi_SampleSample_LoopSnocSample :
     ={glob A, i} ==> ={ res}.
 proof.
 proc; inline *.
-seq 18 18 : (={glob A, glob O_MEFGCMA_WOTSTWES, R_DistRCH_Game23WOTSTW.O_R_DistRCH_Game23WOTSTW_THFC.adl, ps}); last by sim.
-call (:   ={glob O_THFC_Default, glob O_MEFGCMA_WOTSTWES, glob O_DistRCH, R_DistRCH_Game23WOTSTW.O_R_DistRCH_Game23WOTSTW_THFC.adl} 
+seq 18 18 : (={glob A, glob O_MEUFGCMA_WOTSTWES, R_DistRCH_Game23WOTSTW.O_R_DistRCH_Game23WOTSTW_THFC.adl, ps}); last by sim.
+call (:   ={glob O_THFC_Default, glob O_MEUFGCMA_WOTSTWES, glob O_DistRCH, R_DistRCH_Game23WOTSTW.O_R_DistRCH_Game23WOTSTW_THFC.adl} 
        /\ DistRCHi_SampleSample.O_DistRCHi.i{1} = DistRCHi_LoopSnocSample.O_DistRCHi.i{2}) => //=.
 + proc.
   inline{1} 2; inline{2} 2.
@@ -4743,8 +4743,8 @@ local equiv DistRCHi_LoopSnocSample_Alt :
     ={glob A, i} ==> ={ res}.
 proof.
 proc; inline *.
-seq 18 18 : (={glob A, glob O_MEFGCMA_WOTSTWES, R_DistRCH_Game23WOTSTW.O_R_DistRCH_Game23WOTSTW_THFC.adl, ps}); last by sim.
-call (:   ={glob O_THFC_Default, glob O_MEFGCMA_WOTSTWES, glob O_DistRCH, R_DistRCH_Game23WOTSTW.O_R_DistRCH_Game23WOTSTW_THFC.adl} 
+seq 18 18 : (={glob A, glob O_MEUFGCMA_WOTSTWES, R_DistRCH_Game23WOTSTW.O_R_DistRCH_Game23WOTSTW_THFC.adl, ps}); last by sim.
+call (:   ={glob O_THFC_Default, glob O_MEUFGCMA_WOTSTWES, glob O_DistRCH, R_DistRCH_Game23WOTSTW.O_R_DistRCH_Game23WOTSTW_THFC.adl} 
        /\ DistRCHi_LoopSnocSample.O_DistRCHi.i{1} = DistRCHil.O_DistRCHi.i{2}) => //=.
 + proc.
   inline{1} 2; inline{1} 5; inline{2} 2.
@@ -4822,23 +4822,23 @@ local module SM_DT_UD_Cir = {
 
 
 (* - Game-playing proof - *)
-(* Zeroeth step: Show equivalence between M_EF_GCMA_WOTSTWES and Game0_WOTSTWES *)
-local equiv MEFGCMA_Game0_WOTSTWES :
-  M_EF_GCMA_WOTSTWES(A, O_MEFGCMA_WOTSTWES, O_THFC_Default).main ~ Game0_WOTSTWES.main : 
+(* Zeroeth step: Show equivalence between M_EUF_GCMA_WOTSTWES and Game0_WOTSTWES *)
+local equiv MEUFGCMA_Game0_WOTSTWES :
+  M_EUF_GCMA_WOTSTWES(A, O_MEUFGCMA_WOTSTWES, O_THFC_Default).main ~ Game0_WOTSTWES.main : 
     ={glob A} ==> ={res}.
 proof.
 proc; inline *.
-seq 11 11 : (={glob A, O_MEFGCMA_WOTSTWES.qs, O_THFC_Default.tws, ps}); last by sim.
-call (: ={glob O_MEFGCMA_WOTSTWES, glob O_THFC_Default}); [|by proc; inline *; sim | by auto]. 
+seq 11 11 : (={glob A, O_MEUFGCMA_WOTSTWES.qs, O_THFC_Default.tws, ps}); last by sim.
+call (: ={glob O_MEUFGCMA_WOTSTWES, glob O_THFC_Default}); [|by proc; inline *; sim | by auto]. 
 proc; inline *.
 wp => /=.
-while (   ={glob O_MEFGCMA_WOTSTWES, ad, em}
+while (   ={glob O_MEUFGCMA_WOTSTWES, ad, em}
        /\ sig0{1} = sig{2} 
        /\ size sig0{1} <= len 
        /\ size sig{2} <= len
        /\ skWOTS0{1} = insubd sk{2}
        /\ size sk{2} = len
-       /\ ps0{1} = O_MEFGCMA_WOTSTWES.ps{1}).
+       /\ ps0{1} = O_MEUFGCMA_WOTSTWES.ps{1}).
 + by wp; skip => |> &1 lelen_szsig ltlen_szsig; smt(size_rcons DBLL.insubdK).
 wp => /=.
 while{1} (   0 <= size skWOTS3{1} <= len
@@ -4849,20 +4849,20 @@ while{1} (   0 <= size skWOTS3{1} <= len
 + move => _ z.
   by wp; skip => |> *; smt(size_rcons nth_rcons).
 wp => /=.
-while (   ={glob O_MEFGCMA_WOTSTWES}
+while (   ={glob O_MEUFGCMA_WOTSTWES}
        /\ pkWOTS0{1} = pk{2} 
        /\ size pkWOTS0{1} <= len 
        /\ size pk{2} <= len
        /\ size sk{2} = len
        /\ skWOTS2{1} = insubd sk{2}
-       /\ ps2{1} = O_MEFGCMA_WOTSTWES.ps{1}
+       /\ ps2{1} = O_MEUFGCMA_WOTSTWES.ps{1}
        /\ ad1{1} = ad{2}).
 + by wp; skip => |> &1 lelen_szpk ltlen_szpk; smt(size_rcons DBLL.insubdK).
 wp => /=.
-while (   ={glob O_MEFGCMA_WOTSTWES}
+while (   ={glob O_MEUFGCMA_WOTSTWES}
        /\ 0 <= size skWOTS1{1} <= len
-       /\ ss1{1} = O_MEFGCMA_WOTSTWES.ss{2}
-       /\ ps1{1} = O_MEFGCMA_WOTSTWES.ps{1}
+       /\ ss1{1} = O_MEUFGCMA_WOTSTWES.ss{2}
+       /\ ps1{1} = O_MEUFGCMA_WOTSTWES.ps{1}
        /\ skWOTS1{1} = sk{2}
        /\ ad0{1} = ad{2}
        /\ (forall i, 0 <= i < size skWOTS1{1} =>
@@ -4874,9 +4874,9 @@ split => [| *]; [by smt(ge2_len) | split => [/# | *]; rewrite andbA; split; firs
 by congr; apply (eq_from_nth witness) => /#.
 qed.
 
-(* First step: Reduce PRF of prf_sk to distinguishing between Game0_WOTSTWES and- M_EF_GCMA_WOTSTWES without PRF *)
-local lemma Step_Game0_MEFGCMA_WOTSTWES_NOPRF_PRF &m :
-  `|Pr[Game0_WOTSTWES.main() @ &m : res] - Pr[M_EF_GCMA_WOTSTWES(A, O_MEFGCMA_WOTSTWES_NOPRF, O_THFC_Default).main() @ &m : res]|
+(* First step: Reduce PRF of prf_sk to distinguishing between Game0_WOTSTWES and- M_EUF_GCMA_WOTSTWES without PRF *)
+local lemma Step_Game0_MEUFGCMA_WOTSTWES_NOPRF_PRF &m :
+  `|Pr[Game0_WOTSTWES.main() @ &m : res] - Pr[M_EUF_GCMA_WOTSTWES(A, O_MEUFGCMA_WOTSTWES_NOPRF, O_THFC_Default).main() @ &m : res]|
   =
   `|Pr[PRF(R_PRF_Game0NOPRFWOTSTWES(A), O_PRF_Default).main(false) @ &m : res] - Pr[PRF(R_PRF_Game0NOPRFWOTSTWES(A), O_PRF_Default).main(true) @ &m : res]|.
 proof.
@@ -4884,31 +4884,31 @@ do 2! congr; last congr.
 + byequiv => //=.
   proc; inline *.
   wp => /=.
-  seq 11 14 : (={glob A, O_MEFGCMA_WOTSTWES.qs, O_THFC_Default.tws, ps}); last by sim.
-  call (:   ={glob O_THFC_Default, O_MEFGCMA_WOTSTWES.ps, O_MEFGCMA_WOTSTWES.qs} 
+  seq 11 14 : (={glob A, O_MEUFGCMA_WOTSTWES.qs, O_THFC_Default.tws, ps}); last by sim.
+  call (:   ={glob O_THFC_Default, O_MEUFGCMA_WOTSTWES.ps, O_MEUFGCMA_WOTSTWES.qs} 
          /\ O_PRF_Default.b{2} = false
-         /\ O_MEFGCMA_WOTSTWES.ss{1} = O_PRF_Default.k{2}); conseq => />.
+         /\ O_MEUFGCMA_WOTSTWES.ss{1} = O_PRF_Default.k{2}); conseq => />.
   - proc. 
     inline O_PRF_Default.query.
-    seq 3 3 : (={O_MEFGCMA_WOTSTWES.ps, O_MEFGCMA_WOTSTWES.qs, ad, m, sk}); last by sim.
+    seq 3 3 : (={O_MEUFGCMA_WOTSTWES.ps, O_MEUFGCMA_WOTSTWES.qs, ad, m, sk}); last by sim.
     while (   #post 
            /\ O_PRF_Default.b{2} = false
-           /\ O_MEFGCMA_WOTSTWES.ss{1} = O_PRF_Default.k{2}); last by auto.
+           /\ O_MEUFGCMA_WOTSTWES.ss{1} = O_PRF_Default.k{2}); last by auto.
     rcondf{2} 2; first by auto.     
     by wp; skip.
   - by sim. 
   by wp; rnd; wp; rnd; wp; skip.
 byequiv => //=.
-transitivity M_EF_GCMA_WOTSTWES(A, O_MEFGCMA_WOTSTWES_NOPRF_Alt, O_THFC_Default).main
+transitivity M_EUF_GCMA_WOTSTWES(A, O_MEUFGCMA_WOTSTWES_NOPRF_Alt, O_THFC_Default).main
              (={glob A} ==> ={res})
              (arg{2} = true /\ ={glob A} ==> ={res}) => [/# | // | |].             
 + proc.
-  seq 5 5 : (={glob A, O_MEFGCMA_WOTSTWES.qs, O_THFC_Default.tws, ps}); last by sim.
-  call (: ={O_MEFGCMA_WOTSTWES.ps, O_MEFGCMA_WOTSTWES.qs, O_THFC_Default.pp, O_THFC_Default.tws}) => />.
-  - conseq (: ={O_MEFGCMA_WOTSTWES.ps, O_MEFGCMA_WOTSTWES.qs, chad, m} 
+  seq 5 5 : (={glob A, O_MEUFGCMA_WOTSTWES.qs, O_THFC_Default.tws, ps}); last by sim.
+  call (: ={O_MEUFGCMA_WOTSTWES.ps, O_MEUFGCMA_WOTSTWES.qs, O_THFC_Default.pp, O_THFC_Default.tws}) => />.
+  - conseq (: ={O_MEUFGCMA_WOTSTWES.ps, O_MEUFGCMA_WOTSTWES.qs, chad, m} 
               ==> 
-              ={O_MEFGCMA_WOTSTWES.ps, O_MEFGCMA_WOTSTWES.qs, res}) => //.
-    * by apply O_MEFGCMA_WOTSTWES_NOPRF_Orig_Alt.  
+              ={O_MEUFGCMA_WOTSTWES.ps, O_MEUFGCMA_WOTSTWES.qs, res}) => //.
+    * by apply O_MEUFGCMA_WOTSTWES_NOPRF_Orig_Alt.  
   - by proc; sim.
   by inline *; wp; do 2! rnd; skip.
 proc.
@@ -4926,33 +4926,33 @@ conseq (: _
               /\ is_valid{2} /\ is_fresh{2} /\ disj_preffour adlO{2} adlOC{2})))) => [/#|].
 inline{1} 13; inline{1} 12; inline{1} 11; inline{1} 10; inline{1} 7.
 inline{2} 13; inline{2} 12; inline{2} 11; inline{2} 10; inline{2} 7.
-seq 5 5 : ((uniq_preffour (map (fun (q : _ * _ * _ *_) => q.`1) O_MEFGCMA_WOTSTWES.qs{1})
+seq 5 5 : ((uniq_preffour (map (fun (q : _ * _ * _ *_) => q.`1) O_MEUFGCMA_WOTSTWES.qs{1})
            =
-           uniq_preffour (map (fun (q : _ * _ * _ *_) => q.`1) O_MEFGCMA_WOTSTWES.qs{2}))
+           uniq_preffour (map (fun (q : _ * _ * _ *_) => q.`1) O_MEUFGCMA_WOTSTWES.qs{2}))
            /\
-           (uniq_preffour (map (fun (q : _ * _ * _ *_) => q.`1) O_MEFGCMA_WOTSTWES.qs{2})
+           (uniq_preffour (map (fun (q : _ * _ * _ *_) => q.`1) O_MEUFGCMA_WOTSTWES.qs{2})
             =>
-            ={glob A, O_MEFGCMA_WOTSTWES.qs, O_THFC_Default.tws, ps})).
-+ call (: (! (uniq_preffour (map (fun (q : _ * _ * _ *_) => q.`1) O_MEFGCMA_WOTSTWES.qs))),
-              ={glob O_THFC_Default, O_MEFGCMA_WOTSTWES.ps, O_MEFGCMA_WOTSTWES.qs}
+            ={glob A, O_MEUFGCMA_WOTSTWES.qs, O_THFC_Default.tws, ps})).
++ call (: (! (uniq_preffour (map (fun (q : _ * _ * _ *_) => q.`1) O_MEUFGCMA_WOTSTWES.qs))),
+              ={glob O_THFC_Default, O_MEUFGCMA_WOTSTWES.ps, O_MEUFGCMA_WOTSTWES.qs}
            /\ O_PRF_Default.b{2} = true
-           /\ O_MEFGCMA_WOTSTWES.ss{1} = O_PRF_Default.k{2}
-           /\ all is_chtype (map (fun (q : _ * _ * _ * _) => q.`1) O_MEFGCMA_WOTSTWES.qs{1})
+           /\ O_MEUFGCMA_WOTSTWES.ss{1} = O_PRF_Default.k{2}
+           /\ all is_chtype (map (fun (q : _ * _ * _ * _) => q.`1) O_MEUFGCMA_WOTSTWES.qs{1})
            /\ (forall (ad : adrs), 
-                 (get_preffour ad \in (map (fun (q : _ * _ * _ *_) => get_preffour q.`1) O_MEFGCMA_WOTSTWES.qs{2})) 
+                 (get_preffour ad \in (map (fun (q : _ * _ * _ *_) => get_preffour q.`1) O_MEUFGCMA_WOTSTWES.qs{2})) 
                  =>
-                 (exists (ad' : adrs), (O_MEFGCMA_WOTSTWES.ps{2}, ad') \in O_PRF_Default.m{2} /\ get_preffour ad = get_preffour ad'))
+                 (exists (ad' : adrs), (O_MEUFGCMA_WOTSTWES.ps{2}, ad') \in O_PRF_Default.m{2} /\ get_preffour ad = get_preffour ad'))
             /\ (forall (ad : adrs), 
-                 (O_MEFGCMA_WOTSTWES.ps{2}, ad) \in O_PRF_Default.m{2}
+                 (O_MEUFGCMA_WOTSTWES.ps{2}, ad) \in O_PRF_Default.m{2}
                  =>
-                 (get_preffour ad \in (map (fun (q : _ * _ * _ *_) => get_preffour q.`1) O_MEFGCMA_WOTSTWES.qs{2}))),
-           (uniq_preffour (map (fun (q : _ * _ * _ *_) => q.`1) O_MEFGCMA_WOTSTWES.qs{1})
+                 (get_preffour ad \in (map (fun (q : _ * _ * _ *_) => get_preffour q.`1) O_MEUFGCMA_WOTSTWES.qs{2}))),
+           (uniq_preffour (map (fun (q : _ * _ * _ *_) => q.`1) O_MEUFGCMA_WOTSTWES.qs{1})
             =
-            uniq_preffour (map (fun (q : _ * _ * _ *_) => q.`1) O_MEFGCMA_WOTSTWES.qs{2}))) => //=.
+            uniq_preffour (map (fun (q : _ * _ * _ *_) => q.`1) O_MEUFGCMA_WOTSTWES.qs{2}))) => //=.
   - move=> O OC; apply (A_choose_ll O OC).
   - proc.
     sp 1 1; wp => /=.
-    case (get_preffour ad{2} \in map (fun (q : _ * _ * _ *_) => get_preffour q.`1) O_MEFGCMA_WOTSTWES.qs{2}).
+    case (get_preffour ad{2} \in map (fun (q : _ * _ * _ *_) => get_preffour q.`1) O_MEUFGCMA_WOTSTWES.qs{2}).
     * conseq (: _ ==> true) => />. 
       + move=> &2 uqpfqs qsch relqsm relmqs pfadin pk sig m pk' csig'.
         split => [nuqpfrcqs |]. 
@@ -4976,29 +4976,29 @@ seq 5 5 : ((uniq_preffour (map (fun (q : _ * _ * _ *_) => q.`1) O_MEFGCMA_WOTSTW
         conseq (: _ ==> true); first by smt(size_rcons).
         by sp; if{2}; auto. 
       by wp; skip. 
-    while (={ad, sk, sig, em, O_MEFGCMA_WOTSTWES.ps} /\ size sk{1} = len /\ 0 <= size sig{1} <= len).
+    while (={ad, sk, sig, em, O_MEUFGCMA_WOTSTWES.ps} /\ size sk{1} = len /\ 0 <= size sig{1} <= len).
     * wp; skip => />; smt(size_rcons).
     wp.
-    while (={ad, pk, sk, O_MEFGCMA_WOTSTWES.ps} /\ size sk{1} = len /\ 0 <= size pk{1} <= len).
+    while (={ad, pk, sk, O_MEUFGCMA_WOTSTWES.ps} /\ size sk{1} = len /\ 0 <= size pk{1} <= len).
     * wp; skip => />; smt(size_rcons).
     wp => /=.
     exists* O_PRF_Default.m{2}; elim* => m.
     while (   ={ad, sk}
            /\ is_chtype ad{2}
            /\ O_PRF_Default.b{2} = true
-           /\ ! (get_preffour ad{2} \in map (fun (q : adrs * msgWOTS * pkWOTS * sigWOTS) => get_preffour q.`1) O_MEFGCMA_WOTSTWES.qs{2})
+           /\ ! (get_preffour ad{2} \in map (fun (q : adrs * msgWOTS * pkWOTS * sigWOTS) => get_preffour q.`1) O_MEUFGCMA_WOTSTWES.qs{2})
            /\ (forall (ad' : adrs), 
-                 (get_preffour ad' \in (map (fun (q : _ * _ * _ *_) => get_preffour q.`1) O_MEFGCMA_WOTSTWES.qs{2})) 
+                 (get_preffour ad' \in (map (fun (q : _ * _ * _ *_) => get_preffour q.`1) O_MEUFGCMA_WOTSTWES.qs{2})) 
                  =>
-                 (exists (ad'' : adrs), (O_MEFGCMA_WOTSTWES.ps{2}, ad'') \in m /\ get_preffour ad' = get_preffour ad''))
+                 (exists (ad'' : adrs), (O_MEUFGCMA_WOTSTWES.ps{2}, ad'') \in m /\ get_preffour ad' = get_preffour ad''))
            /\ (forall (ad' : adrs),
-                 (O_MEFGCMA_WOTSTWES.ps{2}, ad') \in m 
+                 (O_MEUFGCMA_WOTSTWES.ps{2}, ad') \in m 
                  =>
-                 (get_preffour ad' \in (map (fun (q : _ * _ * _ *_) => get_preffour q.`1) O_MEFGCMA_WOTSTWES.qs{2})))
+                 (get_preffour ad' \in (map (fun (q : _ * _ * _ *_) => get_preffour q.`1) O_MEUFGCMA_WOTSTWES.qs{2})))
            /\ (forall (ad' : adrs), 
-                 (O_MEFGCMA_WOTSTWES.ps{2}, ad') \in O_PRF_Default.m{2} 
+                 (O_MEUFGCMA_WOTSTWES.ps{2}, ad') \in O_PRF_Default.m{2} 
                  <=> 
-                 (((O_MEFGCMA_WOTSTWES.ps{2}, ad') \in m) \/ (ad' \in mkseq (fun (i : int) => set_htbidx (set_chthidx ad{2} i) 0) (size sk{2}))))
+                 (((O_MEUFGCMA_WOTSTWES.ps{2}, ad') \in m) \/ (ad' \in mkseq (fun (i : int) => set_htbidx (set_chthidx ad{2} i) 0) (size sk{2}))))
            /\ 0 <= size sk{2} <= len).
     * inline *.
       rcondt{2} 2; first by auto.
@@ -5068,7 +5068,7 @@ seq 5 5 : ((uniq_preffour (map (fun (q : _ * _ * _ *_) => q.`1) O_MEFGCMA_WOTSTW
   - move=> &1.
     by proc; wp; skip.
   by inline *; wp; rnd; wp; rnd; wp; skip => />; smt(mem_empty ge2_len).
-case (uniq_preffour (map (fun (q : _ * _ * _ *_) => q.`1) O_MEFGCMA_WOTSTWES.qs{2})).
+case (uniq_preffour (map (fun (q : _ * _ * _ *_) => q.`1) O_MEUFGCMA_WOTSTWES.qs{2})).
 + sim => /> /#. 
 wp => /=; conseq (: _ ==> true) => />.
 inline *.
@@ -5082,14 +5082,14 @@ call{1} (: true ==> true); 2: call{2} (: true ==> true); first 2 proc true => //
 by skip; smt(ge2_len).
 qed.
 
-(* Second step: Show equivalence between M_EF_GCMA_WOTSTWES without PRF and Game2_WOTSTWES *)
-local equiv MEFGCMA_WOTSTWES_NOPRF_Game2_WOTSTWES : 
-  M_EF_GCMA_WOTSTWES(A, O_MEFGCMA_WOTSTWES_NOPRF, O_THFC_Default).main ~ Game2_WOTSTWES.main : 
+(* Second step: Show equivalence between M_EUF_GCMA_WOTSTWES without PRF and Game2_WOTSTWES *)
+local equiv MEUFGCMA_WOTSTWES_NOPRF_Game2_WOTSTWES : 
+  M_EUF_GCMA_WOTSTWES(A, O_MEUFGCMA_WOTSTWES_NOPRF, O_THFC_Default).main ~ Game2_WOTSTWES.main : 
     ={glob A} ==> ={res}.
 proof.
 proc; inline *.
-seq 12 12 : (={glob O_MEFGCMA_WOTSTWES, glob O_THFC_Default, ps, i, m', sig'}); last by sim.
-do 2! call (: ={glob O_MEFGCMA_WOTSTWES, glob O_THFC_Default}); [|by proc; inline *; sim | by auto].
+seq 12 12 : (={glob O_MEUFGCMA_WOTSTWES, glob O_THFC_Default, ps, i, m', sig'}); last by sim.
+do 2! call (: ={glob O_MEUFGCMA_WOTSTWES, glob O_THFC_Default}); [|by proc; inline *; sim | by auto].
 proc.
 wp; swap{1} [5..6] -2; swap{2} 6 -1.
 seq 5 5 : (    #pre 
@@ -5102,7 +5102,7 @@ while{1} (   is_chtype ad{1}
           /\ (forall (i : int), 0 <= i < size sig => 
                nth witness sig i 
                = 
-               cf O_MEFGCMA_WOTSTWES.ps (set_chthidx ad i) 0 (BaseW.val em.[i]) (val (nth witness sk i))){1}
+               cf O_MEUFGCMA_WOTSTWES.ps (set_chthidx ad i) 0 (BaseW.val em.[i]) (val (nth witness sk i))){1}
           /\ size sig{1} <= len)
          (len - size sig{1}).
 + move=> _ z.
@@ -5115,7 +5115,7 @@ while{1} (   is_chtype ad{1}
           /\ (forall (i : int), 0 <= i < size pk => 
                 nth witness pk i
                 = 
-                cf O_MEFGCMA_WOTSTWES.ps (set_chthidx ad i) 0 (w - 1) (val (nth witness sk i))){1}
+                cf O_MEUFGCMA_WOTSTWES.ps (set_chthidx ad i) 0 (w - 1) (val (nth witness sk i))){1}
           /\ size pk{1} <= len)
          (len - size pk{1}).
 + move=> _ z.
@@ -5128,7 +5128,7 @@ while{2} (    is_chtype ad{2}
           /\ (forall (i : int), 0 <= i < size pk => 
                 nth witness pk i 
                 =
-                cf O_MEFGCMA_WOTSTWES.ps (set_chthidx ad i) 0 (w - 1) (val (nth witness sk i))){2}
+                cf O_MEUFGCMA_WOTSTWES.ps (set_chthidx ad i) 0 (w - 1) (val (nth witness sk i))){2}
           /\ size pk{2} <= len)
          (len - size pk{2}).
 + move=> _ z.
@@ -5141,7 +5141,7 @@ while{2} (   is_chtype ad{2}
           /\ (forall (i : int), 0 <= i < size sig => 
                 nth witness sig i 
                 = 
-                cf O_MEFGCMA_WOTSTWES.ps (set_chthidx ad i) 0 (BaseW.val em.[i]) (val (nth witness sk i))){2}
+                cf O_MEUFGCMA_WOTSTWES.ps (set_chthidx ad i) 0 (BaseW.val em.[i]) (val (nth witness sk i))){2}
           /\ size sig{2} <= len)
          (len - size sig{2}).
 + move=> _ z.
@@ -5178,25 +5178,25 @@ proof.
 do 2! congr; last congr.
 + byequiv => //.
   proc; inline *.
-  seq 10 16 : (   ={glob A, glob O_THFC_Default, O_MEFGCMA_WOTSTWES.qs, ps}
+  seq 10 16 : (   ={glob A, glob O_THFC_Default, O_MEUFGCMA_WOTSTWES.qs, ps}
               /\ b{2} = false
-              /\ (O_MEFGCMA_WOTSTWES.ps = ps){1}
+              /\ (O_MEUFGCMA_WOTSTWES.ps = ps){1}
               /\ (O_DistRCH.b = b){2}
               /\ (O_DistRCH.ps = ps){2}
               /\ (O_THFC_Default.pp = ps){1}
               /\ (O_THFC_Default.pp = ps){2}
-              /\ O_MEFGCMA_WOTSTWES.qs{1} = []
-              /\ O_MEFGCMA_WOTSTWES.qs{2} = []
+              /\ O_MEUFGCMA_WOTSTWES.qs{1} = []
+              /\ O_MEUFGCMA_WOTSTWES.qs{2} = []
               /\ O_THFC_Default.tws{1} = []
               /\ O_THFC_Default.tws{2} = []
               /\ R_DistRCH_Game23WOTSTW.O_R_DistRCH_Game23WOTSTW_THFC.adl{2} = []).
   - by auto => />.
-  seq 1 1 : (   ={glob A, O_MEFGCMA_WOTSTWES.qs, ps}
+  seq 1 1 : (   ={glob A, O_MEUFGCMA_WOTSTWES.qs, ps}
              /\ O_THFC_Default.tws{1} = R_DistRCH_Game23WOTSTW.O_R_DistRCH_Game23WOTSTW_THFC.adl{2}).
-  - call (:   ={O_MEFGCMA_WOTSTWES.qs, O_THFC_Default.pp} 
+  - call (:   ={O_MEUFGCMA_WOTSTWES.qs, O_THFC_Default.pp} 
            /\ O_DistRCH.b{2} = false
-           /\ O_MEFGCMA_WOTSTWES.ps{1} = O_DistRCH.ps{2}
-           /\ O_MEFGCMA_WOTSTWES.ps{1} = O_THFC_Default.pp{2}
+           /\ O_MEUFGCMA_WOTSTWES.ps{1} = O_DistRCH.ps{2}
+           /\ O_MEUFGCMA_WOTSTWES.ps{1} = O_THFC_Default.pp{2}
            /\ O_THFC_Default.tws{1} = R_DistRCH_Game23WOTSTW.O_R_DistRCH_Game23WOTSTW_THFC.adl{2}).
     * proc; inline *.
       rcondf{2} 6; first by auto.
@@ -5219,7 +5219,7 @@ do 2! congr; last congr.
                   /\ (forall (i : int), 0 <= i < len =>
                        nth witness sig{1} i 
                        = 
-                       cf O_MEFGCMA_WOTSTWES.ps{1} (set_chthidx ad{1} i) 0 (BaseW.val em{1}.[i]) (val (nth witness sk{1} i)))
+                       cf O_MEUFGCMA_WOTSTWES.ps{1} (set_chthidx ad{1} i) 0 (BaseW.val em{1}.[i]) (val (nth witness sk{1} i)))
                   /\ (forall (i : int), 0 <= i < len => 
                        nth witness chal{2} i
                        = 
@@ -5229,8 +5229,8 @@ do 2! congr; last congr.
                /\ ad0{2} = ad{2}
                /\ is_chtype ad{1}
                /\ sk{1} = chal'{2}
-               /\ O_MEFGCMA_WOTSTWES.ps{1} = O_DistRCH.ps{2}
-               /\ O_MEFGCMA_WOTSTWES.ps{1} = O_THFC_Default.pp{2}
+               /\ O_MEUFGCMA_WOTSTWES.ps{1} = O_DistRCH.ps{2}
+               /\ O_MEUFGCMA_WOTSTWES.ps{1} = O_THFC_Default.pp{2}
                /\ ad0{2} = ad{2} 
                /\ m0{2} = m{2} 
                /\ em{1} = em0{2}
@@ -5240,7 +5240,7 @@ do 2! congr; last congr.
                /\ (forall (i : int), 0 <= i < size sig{1} =>
                     nth witness sig{1} i 
                     = 
-                    cf O_MEFGCMA_WOTSTWES.ps{1} (set_chthidx ad{1} i) 0 (BaseW.val em{1}.[i]) (val (nth witness sk{1} i)))
+                    cf O_MEUFGCMA_WOTSTWES.ps{1} (set_chthidx ad{1} i) 0 (BaseW.val em{1}.[i]) (val (nth witness sk{1} i)))
                /\ (forall (i : int), 0 <= i < size chal0{2} => 
                     nth witness chal0{2} i 
                     = 
@@ -5259,8 +5259,8 @@ do 2! congr; last congr.
              /\ sk{1} = chal'{2}
              /\ sk{1} \in ddgstblockl
              /\ chal'{2} \in ddgstblockl
-             /\ O_MEFGCMA_WOTSTWES.ps{1} = O_DistRCH.ps{2}
-             /\ O_MEFGCMA_WOTSTWES.ps{1} = O_THFC_Default.pp{2}
+             /\ O_MEUFGCMA_WOTSTWES.ps{1} = O_DistRCH.ps{2}
+             /\ O_MEUFGCMA_WOTSTWES.ps{1} = O_THFC_Default.pp{2}
              /\ 0 <= size pk{1} <= len
              /\ 0 <= size pk{2} <= len
              /\ 0 <= size sig{2} <= len
@@ -5271,7 +5271,7 @@ do 2! congr; last congr.
              /\ (forall (i : int), 0 <= i < len =>
                   nth witness sig{1} i 
                   = 
-                  cf O_MEFGCMA_WOTSTWES.ps{1} (set_chthidx ad{1} i) 0 (BaseW.val em{1}.[i]) (val (nth witness sk{1} i)))
+                  cf O_MEUFGCMA_WOTSTWES.ps{1} (set_chthidx ad{1} i) 0 (BaseW.val em{1}.[i]) (val (nth witness sk{1} i)))
              /\ (forall (i : int), 0 <= i < len => 
                   nth witness chal{2} i 
                   = 
@@ -5287,8 +5287,8 @@ do 2! congr; last congr.
                 /\ sk{1} = chal'{2}
                 /\ sk{1} \in ddgstblockl
                 /\ chal'{2} \in ddgstblockl
-                /\ O_MEFGCMA_WOTSTWES.ps{1} = O_DistRCH.ps{2}
-                /\ O_MEFGCMA_WOTSTWES.ps{1} = O_THFC_Default.pp{2}
+                /\ O_MEUFGCMA_WOTSTWES.ps{1} = O_DistRCH.ps{2}
+                /\ O_MEUFGCMA_WOTSTWES.ps{1} = O_THFC_Default.pp{2}
                 /\ 0 <= size pk{1} < len
                 /\ 0 <= size pk{2} < len
                 /\ 0 <= size sig{2} < len
@@ -5296,7 +5296,7 @@ do 2! congr; last congr.
                 /\ (forall (i : int), 0 <= i < len =>
                       nth witness sig{1} i 
                       = 
-                      cf O_MEFGCMA_WOTSTWES.ps{1} (set_chthidx ad{1} i) 0 (BaseW.val em{1}.[i]) (val (nth witness sk{1} i)))
+                      cf O_MEUFGCMA_WOTSTWES.ps{1} (set_chthidx ad{1} i) 0 (BaseW.val em{1}.[i]) (val (nth witness sk{1} i)))
                 /\ (forall (i : int), 0 <= i < len => 
                      nth witness chal{2} i 
                      =
@@ -5358,31 +5358,31 @@ do 2! congr; last congr.
       by auto.
     by skip.
   wp => /=.
-  by sim : (   ={m, m', i, O_MEFGCMA_WOTSTWES.qs}
+  by sim : (   ={m, m', i, O_MEUFGCMA_WOTSTWES.qs}
             /\ pkWOTS0{1} = pkWOTS{2}
             /\ pkWOTS1{1} = pkWOTS0{2}
             /\ O_THFC_Default.tws{1} = R_DistRCH_Game23WOTSTW.O_R_DistRCH_Game23WOTSTW_THFC.adl{2}).
 byequiv => //.
 proc; inline *.
-seq 10 16 : (   ={glob A, glob O_THFC_Default, O_MEFGCMA_WOTSTWES.qs, ps}
+seq 10 16 : (   ={glob A, glob O_THFC_Default, O_MEUFGCMA_WOTSTWES.qs, ps}
              /\ b{2} = true
-             /\ (O_MEFGCMA_WOTSTWES.ps = ps){1}
+             /\ (O_MEUFGCMA_WOTSTWES.ps = ps){1}
              /\ (O_DistRCH.b = b){2}
              /\ (O_DistRCH.ps = ps){2}
              /\ (O_THFC_Default.pp = ps){1}
              /\ (O_THFC_Default.pp = ps){2}
-             /\ O_MEFGCMA_WOTSTWES.qs{1} = []
-             /\ O_MEFGCMA_WOTSTWES.qs{2} = []
+             /\ O_MEUFGCMA_WOTSTWES.qs{1} = []
+             /\ O_MEUFGCMA_WOTSTWES.qs{2} = []
              /\ O_THFC_Default.tws{1} = []
              /\ O_THFC_Default.tws{2} = []
              /\ R_DistRCH_Game23WOTSTW.O_R_DistRCH_Game23WOTSTW_THFC.adl{2} = []).
 + by auto => />.
-seq 1 1 : (   ={glob A, O_MEFGCMA_WOTSTWES.qs, ps}
+seq 1 1 : (   ={glob A, O_MEUFGCMA_WOTSTWES.qs, ps}
            /\ O_THFC_Default.tws{1} = R_DistRCH_Game23WOTSTW.O_R_DistRCH_Game23WOTSTW_THFC.adl{2}).
-+ call (:   ={O_MEFGCMA_WOTSTWES.qs, O_THFC_Default.pp} 
++ call (:   ={O_MEUFGCMA_WOTSTWES.qs, O_THFC_Default.pp} 
          /\ O_DistRCH.b{2} = true
-         /\ O_MEFGCMA_WOTSTWES.ps{1} = O_DistRCH.ps{2}
-         /\ O_MEFGCMA_WOTSTWES.ps{1} = O_THFC_Default.pp{2}
+         /\ O_MEUFGCMA_WOTSTWES.ps{1} = O_DistRCH.ps{2}
+         /\ O_MEUFGCMA_WOTSTWES.ps{1} = O_THFC_Default.pp{2}
          /\ O_THFC_Default.tws{1} = R_DistRCH_Game23WOTSTW.O_R_DistRCH_Game23WOTSTW_THFC.adl{2}).
   - proc; inline *.
     rcondt{2} 6; first by auto.
@@ -5407,7 +5407,7 @@ seq 1 1 : (   ={glob A, O_MEFGCMA_WOTSTWES.qs, ps}
                     nth witness sig{1} i 
                     = 
                     if BaseW.val em{1}.[i] <> 0
-                    then cf O_MEFGCMA_WOTSTWES.ps{1} (set_chthidx ad{1} i) (BaseW.val em{1}.[i] - 1) 1 (val (nth witness sk{1} i))
+                    then cf O_MEUFGCMA_WOTSTWES.ps{1} (set_chthidx ad{1} i) (BaseW.val em{1}.[i] - 1) 1 (val (nth witness sk{1} i))
                     else nth witness sk{1} i)).
     * while{1} (   ={m, ad, pk, em}
                /\ is_chtype ad{1}
@@ -5415,14 +5415,14 @@ seq 1 1 : (   ={glob A, O_MEFGCMA_WOTSTWES.qs, ps}
                /\ em{2} = encode_msgWOTS m{2}
                /\ sk{1} = chal'{2}
                /\ chal{2} = chal'{2}
-               /\ O_MEFGCMA_WOTSTWES.ps{1} = O_DistRCH.ps{2}
-               /\ O_MEFGCMA_WOTSTWES.ps{1} = O_THFC_Default.pp{2}
+               /\ O_MEUFGCMA_WOTSTWES.ps{1} = O_DistRCH.ps{2}
+               /\ O_MEUFGCMA_WOTSTWES.ps{1} = O_THFC_Default.pp{2}
                /\ 0 <= size sig{1} <= len
                /\ (forall (i : int), 0 <= i < size sig{1} =>
                     nth witness sig{1} i 
                     = 
                     if BaseW.val em{1}.[i] <> 0
-                    then cf O_MEFGCMA_WOTSTWES.ps{1} (set_chthidx ad{1} i) (BaseW.val em{1}.[i] - 1) 1 (val (nth witness sk{1} i))
+                    then cf O_MEUFGCMA_WOTSTWES.ps{1} (set_chthidx ad{1} i) (BaseW.val em{1}.[i] - 1) 1 (val (nth witness sk{1} i))
                     else nth witness sk{1} i))
              (len - size sig{1}); last first.
       + wp; skip => /> &2 adch chalin.
@@ -5441,8 +5441,8 @@ seq 1 1 : (   ={glob A, O_MEFGCMA_WOTSTWES.qs, ps}
            /\ chal{2} = chal'{2}
            /\ sk{1} \in ddgstblockl
            /\ chal'{2} \in ddgstblockl
-           /\ O_MEFGCMA_WOTSTWES.ps{1} = O_DistRCH.ps{2}
-           /\ O_MEFGCMA_WOTSTWES.ps{1} = O_THFC_Default.pp{2}
+           /\ O_MEUFGCMA_WOTSTWES.ps{1} = O_DistRCH.ps{2}
+           /\ O_MEUFGCMA_WOTSTWES.ps{1} = O_THFC_Default.pp{2}
            /\ 0 <= size pk{1} <= len
            /\ 0 <= size pk{2} <= len
            /\ 0 <= size sig{2} <= len
@@ -5453,7 +5453,7 @@ seq 1 1 : (   ={glob A, O_MEFGCMA_WOTSTWES.qs, ps}
                 nth witness sig{1} i 
                 = 
                 if BaseW.val em{1}.[i] <> 0
-                then cf O_MEFGCMA_WOTSTWES.ps{1} (set_chthidx ad{1} i) (BaseW.val em{1}.[i] - 1) 1 (val (nth witness sk{1} i))
+                then cf O_MEUFGCMA_WOTSTWES.ps{1} (set_chthidx ad{1} i) (BaseW.val em{1}.[i] - 1) 1 (val (nth witness sk{1} i))
                 else nth witness sk{1} i)
            /\ (forall (i : int), 0 <= i < size sig{2} => 
                  nth witness sig{1} i = nth witness sig{2} i)); last first.
@@ -5467,8 +5467,8 @@ seq 1 1 : (   ={glob A, O_MEFGCMA_WOTSTWES.qs, ps}
               /\ chal{2} = chal'{2}
               /\ sk{1} \in ddgstblockl
               /\ chal'{2} \in ddgstblockl
-              /\ O_MEFGCMA_WOTSTWES.ps{1} = O_DistRCH.ps{2}
-              /\ O_MEFGCMA_WOTSTWES.ps{1} = O_THFC_Default.pp{2}
+              /\ O_MEUFGCMA_WOTSTWES.ps{1} = O_DistRCH.ps{2}
+              /\ O_MEUFGCMA_WOTSTWES.ps{1} = O_THFC_Default.pp{2}
               /\ 0 <= size pk{1} < len
               /\ 0 <= size pk{2} < len
               /\ 0 <= size sig{2} < len
@@ -5476,7 +5476,7 @@ seq 1 1 : (   ={glob A, O_MEFGCMA_WOTSTWES.qs, ps}
               /\ (forall (i : int), 0 <= i < size sig{1} =>
                     nth witness sig{1} i = 
                     if BaseW.val em{1}.[i] <> 0
-                    then cf O_MEFGCMA_WOTSTWES.ps{1} (set_chthidx ad{1} i) (BaseW.val em{1}.[i] - 1) 1 (val (nth witness sk{1} i))
+                    then cf O_MEUFGCMA_WOTSTWES.ps{1} (set_chthidx ad{1} i) (BaseW.val em{1}.[i] - 1) 1 (val (nth witness sk{1} i))
                     else nth witness sk{1} i)
               /\ (forall (i : int), 0 <= i < size sig{2} => 
                     nth witness sig{1} i = nth witness sig{2} i)
@@ -5522,7 +5522,7 @@ seq 1 1 : (   ={glob A, O_MEFGCMA_WOTSTWES.qs, ps}
     by auto.
   by skip.
 wp => /=.
-by sim : (   ={m, m', i, O_MEFGCMA_WOTSTWES.qs}
+by sim : (   ={m, m', i, O_MEUFGCMA_WOTSTWES.qs}
           /\ pkWOTS0{1} = pkWOTS{2}
           /\ pkWOTS1{1} = pkWOTS0{2}
           /\ O_THFC_Default.tws{1} = R_DistRCH_Game23WOTSTW.O_R_DistRCH_Game23WOTSTW_THFC.adl{2}).
@@ -5547,7 +5547,7 @@ have ->:
                  (={glob A, i} ==> ={res}) => [/# | // | |]; last first.
     * by apply DistRCHi_Orig_Alt.
     proc; inline *. 
-    seq 16 17: (   ={glob A, glob O_MEFGCMA_WOTSTWES, glob O_THFC_Default, O_DistRCH.ps, R_DistRCH_Game23WOTSTW.O_R_DistRCH_Game23WOTSTW_THFC.adl, ps}
+    seq 16 17: (   ={glob A, glob O_MEUFGCMA_WOTSTWES, glob O_THFC_Default, O_DistRCH.ps, R_DistRCH_Game23WOTSTW.O_R_DistRCH_Game23WOTSTW_THFC.adl, ps}
                 /\ b{1} = false
                 /\ i{2} = 0
                 /\ O_DistRCH.b{1} = b{1}
@@ -5555,10 +5555,10 @@ have ->:
                 /\ O_THFC_Default.pp{1} = ps{1}
                 /\ O_DistRCH.ps{1} = ps{1}
                 /\ O_THFC_Default.tws{1} = []
-                /\ O_MEFGCMA_WOTSTWES.qs{1} = []
+                /\ O_MEUFGCMA_WOTSTWES.qs{1} = []
                 /\ R_DistRCH_Game23WOTSTW.O_R_DistRCH_Game23WOTSTW_THFC.adl{1} = []); first by auto.
-    seq 1 1 : (={glob A, O_MEFGCMA_WOTSTWES.qs, R_DistRCH_Game23WOTSTW.O_R_DistRCH_Game23WOTSTW_THFC.adl, ps}); last by sim.
-    call (:   ={O_MEFGCMA_WOTSTWES.qs, O_THFC_Default.pp, O_DistRCH.ps, R_DistRCH_Game23WOTSTW.O_R_DistRCH_Game23WOTSTW_THFC.adl}
+    seq 1 1 : (={glob A, O_MEUFGCMA_WOTSTWES.qs, R_DistRCH_Game23WOTSTW.O_R_DistRCH_Game23WOTSTW_THFC.adl, ps}); last by sim.
+    call (:   ={O_MEUFGCMA_WOTSTWES.qs, O_THFC_Default.pp, O_DistRCH.ps, R_DistRCH_Game23WOTSTW.O_R_DistRCH_Game23WOTSTW_THFC.adl}
            /\ O_DistRCH.b{1} = false
            /\ DistRCHi.O_DistRCHi.i{2} = 0) => //; last first.
     * by proc => />; sim.
@@ -5571,7 +5571,7 @@ have ->:
                (={glob A, i} ==> ={res}) => [/# | // | |]; last first.
   * by apply DistRCHi_Orig_Alt.
   proc; inline *.
-  seq 16 17: (   ={glob A, glob O_MEFGCMA_WOTSTWES, glob O_THFC_Default, O_DistRCH.ps, R_DistRCH_Game23WOTSTW.O_R_DistRCH_Game23WOTSTW_THFC.adl, ps}
+  seq 16 17: (   ={glob A, glob O_MEUFGCMA_WOTSTWES, glob O_THFC_Default, O_DistRCH.ps, R_DistRCH_Game23WOTSTW.O_R_DistRCH_Game23WOTSTW_THFC.adl, ps}
               /\ b{1} = true
               /\ i{2} = w - 2
               /\ O_DistRCH.b{1} = b{1}
@@ -5579,10 +5579,10 @@ have ->:
               /\ O_THFC_Default.pp{1} = ps{1}
               /\ O_DistRCH.ps{1} = ps{1}
               /\ O_THFC_Default.tws{1} = []
-              /\ O_MEFGCMA_WOTSTWES.qs{1} = []
+              /\ O_MEUFGCMA_WOTSTWES.qs{1} = []
               /\ R_DistRCH_Game23WOTSTW.O_R_DistRCH_Game23WOTSTW_THFC.adl{1} = []); first by auto.
-  seq 1 1 : (={glob A, O_MEFGCMA_WOTSTWES.qs, R_DistRCH_Game23WOTSTW.O_R_DistRCH_Game23WOTSTW_THFC.adl, ps}); last by sim.
-  call (:   ={O_MEFGCMA_WOTSTWES.qs, O_THFC_Default.pp, O_DistRCH.ps, R_DistRCH_Game23WOTSTW.O_R_DistRCH_Game23WOTSTW_THFC.adl}
+  seq 1 1 : (={glob A, O_MEUFGCMA_WOTSTWES.qs, R_DistRCH_Game23WOTSTW.O_R_DistRCH_Game23WOTSTW_THFC.adl, ps}); last by sim.
+  call (:   ={O_MEUFGCMA_WOTSTWES.qs, O_THFC_Default.pp, O_DistRCH.ps, R_DistRCH_Game23WOTSTW.O_R_DistRCH_Game23WOTSTW_THFC.adl}
          /\ O_DistRCH.b{1} = true
          /\ DistRCHi.O_DistRCHi.i{2} = w - 2) => //; last first.
   - by proc => />; sim.
@@ -5630,7 +5630,7 @@ have ->:
   - byequiv => //.
     proc => /=; inline{1} 6.
     wp; inline{1} 5; inline{2} 5; inline{2} 6; inline{2} 4; inline{2} 7.
-    seq 6 8 : (   ={glob A, glob O_MEFGCMA_WOTSTWES, glob O_THFC_Default, R_DistRCH_Game23WOTSTW.O_R_DistRCH_Game23WOTSTW_THFC.adl, O_DistRCH.b, i}
+    seq 6 8 : (   ={glob A, glob O_MEUFGCMA_WOTSTWES, glob O_THFC_Default, R_DistRCH_Game23WOTSTW.O_R_DistRCH_Game23WOTSTW_THFC.adl, O_DistRCH.b, i}
                /\ i{1} = k
                /\ b{2} = false
                /\ ps{1} = pp{2}
@@ -5640,49 +5640,49 @@ have ->:
                /\ O_DistRCH.ps{1} = ps{1}
                /\ O_THFC_Default.pp{1} = ps{1}
                /\ O_SMDTUD_Default.pp{2} = pp{2}
-               /\ O_MEFGCMA_WOTSTWES.qs{1} = [] 
+               /\ O_MEUFGCMA_WOTSTWES.qs{1} = [] 
                /\ O_THFC_Default.tws{1} = []
                /\ O_SMDTUD_Default.ts{2} = []
                /\ R_DistRCH_Game23WOTSTW.O_R_DistRCH_Game23WOTSTW_THFC.adl{1} = []).
     * by inline *; auto.
-    seq 1 2 : (   ={glob A, glob O_MEFGCMA_WOTSTWES, O_THFC_Default.pp, R_DistRCH_Game23WOTSTW.O_R_DistRCH_Game23WOTSTW_THFC.adl, ps}
-               /\ all is_chtype (map (fun (admpksig : adrs * msgWOTS * pkWOTS * sigWOTS) => admpksig.`1) O_MEFGCMA_WOTSTWES.qs{1})
-               /\ O_SMDTUD_Default.ts{2} = relcqsad_udi O_MEFGCMA_WOTSTWES.qs{1} k
+    seq 1 2 : (   ={glob A, glob O_MEUFGCMA_WOTSTWES, O_THFC_Default.pp, R_DistRCH_Game23WOTSTW.O_R_DistRCH_Game23WOTSTW_THFC.adl, ps}
+               /\ all is_chtype (map (fun (admpksig : adrs * msgWOTS * pkWOTS * sigWOTS) => admpksig.`1) O_MEUFGCMA_WOTSTWES.qs{1})
+               /\ O_SMDTUD_Default.ts{2} = relcqsad_udi O_MEUFGCMA_WOTSTWES.qs{1} k
                /\ all (fun (ad : adrs) => 
                          ad \in R_DistRCH_Game23WOTSTW.O_R_DistRCH_Game23WOTSTW_THFC.adl{2} 
-                         \/ ad \in reltqsad_udi O_MEFGCMA_WOTSTWES.qs{1} k) 
+                         \/ ad \in reltqsad_udi O_MEUFGCMA_WOTSTWES.qs{1} k) 
                          O_THFC_Default.tws{2}).
     * wp => /=.
-      call (:   ={glob O_MEFGCMA_WOTSTWES, O_THFC_Default.pp, R_DistRCH_Game23WOTSTW.O_R_DistRCH_Game23WOTSTW_THFC.adl, O_DistRCH.b}
+      call (:   ={glob O_MEUFGCMA_WOTSTWES, O_THFC_Default.pp, R_DistRCH_Game23WOTSTW.O_R_DistRCH_Game23WOTSTW_THFC.adl, O_DistRCH.b}
              /\ O_DistRCH.ps{1} = O_SMDTUD_Default.pp{2}
              /\ O_SMDTUD_Default.pp{2} = O_THFC_Default.pp{2} 
              /\ O_SMDTUD_Default.b{2} = false
              /\ DistRCHil.O_DistRCHi.i{1} = k
              /\ R_SMDTUDC_DistRCHil.O_R_SMDTUDC_DistRCHil.i{2} = k
-             /\ all is_chtype (map (fun (admpksig : adrs * msgWOTS * pkWOTS * sigWOTS) => admpksig.`1) O_MEFGCMA_WOTSTWES.qs{1})
-             /\ O_SMDTUD_Default.ts{2} = relcqsad_udi O_MEFGCMA_WOTSTWES.qs{1} k
+             /\ all is_chtype (map (fun (admpksig : adrs * msgWOTS * pkWOTS * sigWOTS) => admpksig.`1) O_MEUFGCMA_WOTSTWES.qs{1})
+             /\ O_SMDTUD_Default.ts{2} = relcqsad_udi O_MEUFGCMA_WOTSTWES.qs{1} k
              /\ all (fun (ad : adrs) => 
                          ad \in R_DistRCH_Game23WOTSTW.O_R_DistRCH_Game23WOTSTW_THFC.adl{2} 
-                         \/ ad \in reltqsad_udi O_MEFGCMA_WOTSTWES.qs{1} k) 
+                         \/ ad \in reltqsad_udi O_MEUFGCMA_WOTSTWES.qs{1} k) 
                          O_THFC_Default.tws{2}); last by auto.
       + proc.
-        seq 2 2 : (   ={glob O_MEFGCMA_WOTSTWES, O_THFC_Default.pp, R_DistRCH_Game23WOTSTW.O_R_DistRCH_Game23WOTSTW_THFC.adl, O_DistRCH.b, ad, m, chal}
+        seq 2 2 : (   ={glob O_MEUFGCMA_WOTSTWES, O_THFC_Default.pp, R_DistRCH_Game23WOTSTW.O_R_DistRCH_Game23WOTSTW_THFC.adl, O_DistRCH.b, ad, m, chal}
                    /\ is_chtype ad{1}
                    /\ O_DistRCH.ps{1} = O_SMDTUD_Default.pp{2}
                    /\ O_SMDTUD_Default.pp{2} = O_THFC_Default.pp{2}
                    /\ O_SMDTUD_Default.b{2} = false
                    /\ DistRCHil.O_DistRCHi.i{1} = k
                    /\ R_SMDTUDC_DistRCHil.O_R_SMDTUDC_DistRCHil.i{2} = k
-                   /\ all is_chtype (map (fun (admpksig : adrs * msgWOTS * pkWOTS * sigWOTS) => admpksig.`1) O_MEFGCMA_WOTSTWES.qs{1})
-                   /\ O_SMDTUD_Default.ts{2} = relcqsad_udi (rcons O_MEFGCMA_WOTSTWES.qs{1} (ad{2}, m{2}, insubd pk{2}, insubd sig{2})) k
+                   /\ all is_chtype (map (fun (admpksig : adrs * msgWOTS * pkWOTS * sigWOTS) => admpksig.`1) O_MEUFGCMA_WOTSTWES.qs{1})
+                   /\ O_SMDTUD_Default.ts{2} = relcqsad_udi (rcons O_MEUFGCMA_WOTSTWES.qs{1} (ad{2}, m{2}, insubd pk{2}, insubd sig{2})) k
                    /\ all (fun (ad' : adrs) => 
                                ad' \in R_DistRCH_Game23WOTSTW.O_R_DistRCH_Game23WOTSTW_THFC.adl{2} 
-                               \/ ad' \in reltqsad_udi (rcons O_MEFGCMA_WOTSTWES.qs{1} (ad{2}, m{2}, insubd pk{2}, insubd sig{2})) k) 
+                               \/ ad' \in reltqsad_udi (rcons O_MEUFGCMA_WOTSTWES.qs{1} (ad{2}, m{2}, insubd pk{2}, insubd sig{2})) k) 
                                O_THFC_Default.tws{2}
                    /\ size chal{1} = len).
         - inline *; swap{1} 7 -2.
           wp => /=.
-          while (   ={glob O_MEFGCMA_WOTSTWES, O_THFC_Default.pp, R_DistRCH_Game23WOTSTW.O_R_DistRCH_Game23WOTSTW_THFC.adl, O_DistRCH.b, ad, m, ad0, m0, em0, chal0}
+          while (   ={glob O_MEUFGCMA_WOTSTWES, O_THFC_Default.pp, R_DistRCH_Game23WOTSTW.O_R_DistRCH_Game23WOTSTW_THFC.adl, O_DistRCH.b, ad, m, ad0, m0, em0, chal0}
                  /\ ad0{1} = ad{1}
                  /\ m0{1} = m{1}
                  /\ em0{1} = encode_msgWOTS m0{1}
@@ -5692,11 +5692,11 @@ have ->:
                  /\ O_SMDTUD_Default.b{2} = false
                  /\ DistRCHil.O_DistRCHi.i{1} = k
                  /\ R_SMDTUDC_DistRCHil.O_R_SMDTUDC_DistRCHil.i{2} = k
-                 /\ all is_chtype (map (fun (admpksig : adrs * msgWOTS * pkWOTS * sigWOTS) => admpksig.`1) O_MEFGCMA_WOTSTWES.qs{1})
-                 /\ O_SMDTUD_Default.ts{2} = relcqsad_udi (rcons O_MEFGCMA_WOTSTWES.qs{1} (ad{2}, m{2}, insubd pk{2}, insubd sig{2})) k
+                 /\ all is_chtype (map (fun (admpksig : adrs * msgWOTS * pkWOTS * sigWOTS) => admpksig.`1) O_MEUFGCMA_WOTSTWES.qs{1})
+                 /\ O_SMDTUD_Default.ts{2} = relcqsad_udi (rcons O_MEUFGCMA_WOTSTWES.qs{1} (ad{2}, m{2}, insubd pk{2}, insubd sig{2})) k
                  /\ all (fun (ad' : adrs) => 
                              ad' \in R_DistRCH_Game23WOTSTW.O_R_DistRCH_Game23WOTSTW_THFC.adl{2} 
-                             \/ ad' \in reltqsad_udi (rcons O_MEFGCMA_WOTSTWES.qs{1} (ad{2}, m{2}, insubd pk{2}, insubd sig{2})) k) 
+                             \/ ad' \in reltqsad_udi (rcons O_MEUFGCMA_WOTSTWES.qs{1} (ad{2}, m{2}, insubd pk{2}, insubd sig{2})) k) 
                              O_THFC_Default.tws{2}
                  /\ (forall (i : int), 0 <= i < len =>
                        nth witness chal'{2} i
@@ -5722,7 +5722,7 @@ have ->:
                       /\ chal_ele0{2} = cf O_THFC_Default.pp{2} (set_chthidx ad0{2} (size chal0{2})) (R_SMDTUDC_DistRCHil.O_R_SMDTUDC_DistRCHil.i{2} + 1) (j0{2} - 1) (val (nth witness chal'{2} (size chal0{2})))
                       /\ all (fun (ad' : adrs) => 
                              ad' \in R_DistRCH_Game23WOTSTW.O_R_DistRCH_Game23WOTSTW_THFC.adl{2} 
-                             \/ ad' \in reltqsad_udi (rcons O_MEFGCMA_WOTSTWES.qs{1} (ad{2}, m{2}, insubd pk{2}, insubd sig{2})) k) 
+                             \/ ad' \in reltqsad_udi (rcons O_MEUFGCMA_WOTSTWES.qs{1} (ad{2}, m{2}, insubd pk{2}, insubd sig{2})) k) 
                              O_THFC_Default.tws{2}
                       /\ size chal'{2} = len
                       /\ 0 <= size chal0{2} < len
@@ -5751,7 +5751,7 @@ have ->:
             rewrite leem1k_j /= {1}(: em1k = 1 + (em1k - 1)) // /cf => ->.
             by rewrite ch_comp 1:ischtype_setchidx 3:valP //; smt(BaseW.valP).
           wp => /=.
-          while (   ={glob O_MEFGCMA_WOTSTWES, O_THFC_Default.pp, R_DistRCH_Game23WOTSTW.O_R_DistRCH_Game23WOTSTW_THFC.adl, O_DistRCH.b, ad, m, ad0, m0, em0}
+          while (   ={glob O_MEUFGCMA_WOTSTWES, O_THFC_Default.pp, R_DistRCH_Game23WOTSTW.O_R_DistRCH_Game23WOTSTW_THFC.adl, O_DistRCH.b, ad, m, ad0, m0, em0}
                      /\ ad0{1} = ad{1}
                      /\ m0{1} = m{1}
                      /\ em0{1} = encode_msgWOTS m0{1}
@@ -5761,14 +5761,14 @@ have ->:
                      /\ O_SMDTUD_Default.b{2} = false
                      /\ DistRCHil.O_DistRCHi.i{1} = k
                      /\ R_SMDTUDC_DistRCHil.O_R_SMDTUDC_DistRCHil.i{2} = k
-                     /\ all is_chtype (map (fun (admpksig : adrs * msgWOTS * pkWOTS * sigWOTS) => admpksig.`1) O_MEFGCMA_WOTSTWES.qs{1})
+                     /\ all is_chtype (map (fun (admpksig : adrs * msgWOTS * pkWOTS * sigWOTS) => admpksig.`1) O_MEUFGCMA_WOTSTWES.qs{1})
                      /\ O_SMDTUD_Default.ts{2} 
                         = 
-                        relcqsad_udi O_MEFGCMA_WOTSTWES.qs{1} k 
+                        relcqsad_udi O_MEUFGCMA_WOTSTWES.qs{1} k 
                         ++ relcqsad_udi_outer ad0{2} m0{2} k (size chal'{2})
                      /\ all (fun (ad' : adrs) => 
                                  ad' \in R_DistRCH_Game23WOTSTW.O_R_DistRCH_Game23WOTSTW_THFC.adl{2} 
-                                 \/ ad' \in reltqsad_udi (rcons O_MEFGCMA_WOTSTWES.qs{1} (ad{2}, m{2}, insubd pk{2}, insubd sig{2})) k) 
+                                 \/ ad' \in reltqsad_udi (rcons O_MEUFGCMA_WOTSTWES.qs{1} (ad{2}, m{2}, insubd pk{2}, insubd sig{2})) k) 
                                  O_THFC_Default.tws{2}
                      /\ (forall (i : int), 0 <= i < size chal'{2} =>
                            nth witness chal'{2} i
@@ -5886,15 +5886,15 @@ have ->:
     split; last by apply uniq_relcqsadudi => /#.
     rewrite andbC; split; first split => [| _].
     * by smt(relcqsadudi_rng).
-    * apply (IntOrder.ler_trans (size O_MEFGCMA_WOTSTWES.qs{2} * len)); first by smt(relcqsadudi_rng).
+    * apply (IntOrder.ler_trans (size O_MEUFGCMA_WOTSTWES.qs{2} * len)); first by smt(relcqsadudi_rng).
       by rewrite ler_pmul //; smt(ge2_len).
-    apply (djl_parts _ _ R_DistRCH_Game23WOTSTW.O_R_DistRCH_Game23WOTSTW_THFC.adl{2} (reltqsad_udi O_MEFGCMA_WOTSTWES.qs{2} k)) => //. 
+    apply (djl_parts _ _ R_DistRCH_Game23WOTSTW.O_R_DistRCH_Game23WOTSTW_THFC.adl{2} (reltqsad_udi O_MEUFGCMA_WOTSTWES.qs{2} k)) => //. 
     * by apply disj_relcqsadudi => /#.
     by apply disj_relcqsadudi_reltqsadudi => /#.
   byequiv => //.
   proc => /=; inline{1} 6.
   wp; inline{1} 5; inline{2} 5; inline{2} 6; inline{2} 4; inline{2} 7.
-  seq 6 8 : (   ={glob A, glob O_MEFGCMA_WOTSTWES, glob O_THFC_Default, R_DistRCH_Game23WOTSTW.O_R_DistRCH_Game23WOTSTW_THFC.adl, O_DistRCH.b}
+  seq 6 8 : (   ={glob A, glob O_MEUFGCMA_WOTSTWES, glob O_THFC_Default, R_DistRCH_Game23WOTSTW.O_R_DistRCH_Game23WOTSTW_THFC.adl, O_DistRCH.b}
              /\ i{1} = k + 1
              /\ i{2} = k
              /\ b{2} = true
@@ -5905,48 +5905,48 @@ have ->:
              /\ O_DistRCH.ps{1} = ps{1}
              /\ O_THFC_Default.pp{1} = ps{1}
              /\ O_SMDTUD_Default.pp{2} = pp{2}
-             /\ O_MEFGCMA_WOTSTWES.qs{1} = [] 
+             /\ O_MEUFGCMA_WOTSTWES.qs{1} = [] 
              /\ O_THFC_Default.tws{1} = []
              /\ O_SMDTUD_Default.ts{2} = []
              /\ R_DistRCH_Game23WOTSTW.O_R_DistRCH_Game23WOTSTW_THFC.adl{1} = []).
   * by inline *; auto.
-  seq 1 2 : (   ={glob A, glob O_MEFGCMA_WOTSTWES, R_DistRCH_Game23WOTSTW.O_R_DistRCH_Game23WOTSTW_THFC.adl, ps}
-             /\ all is_chtype (map (fun (admpksig : adrs * msgWOTS * pkWOTS * sigWOTS) => admpksig.`1) O_MEFGCMA_WOTSTWES.qs{1})
-             /\ O_SMDTUD_Default.ts{2} = relcqsad_udi O_MEFGCMA_WOTSTWES.qs{1} k
+  seq 1 2 : (   ={glob A, glob O_MEUFGCMA_WOTSTWES, R_DistRCH_Game23WOTSTW.O_R_DistRCH_Game23WOTSTW_THFC.adl, ps}
+             /\ all is_chtype (map (fun (admpksig : adrs * msgWOTS * pkWOTS * sigWOTS) => admpksig.`1) O_MEUFGCMA_WOTSTWES.qs{1})
+             /\ O_SMDTUD_Default.ts{2} = relcqsad_udi O_MEUFGCMA_WOTSTWES.qs{1} k
              /\ all (fun (ad : adrs) => 
-                       ad \in R_DistRCH_Game23WOTSTW.O_R_DistRCH_Game23WOTSTW_THFC.adl{2} \/ ad \in reltqsad_udi O_MEFGCMA_WOTSTWES.qs{1} k) 
+                       ad \in R_DistRCH_Game23WOTSTW.O_R_DistRCH_Game23WOTSTW_THFC.adl{2} \/ ad \in reltqsad_udi O_MEUFGCMA_WOTSTWES.qs{1} k) 
                        O_THFC_Default.tws{2}).
   * wp => /=.
-    call (:   ={glob O_MEFGCMA_WOTSTWES, O_THFC_Default.pp, R_DistRCH_Game23WOTSTW.O_R_DistRCH_Game23WOTSTW_THFC.adl, O_DistRCH.b}
+    call (:   ={glob O_MEUFGCMA_WOTSTWES, O_THFC_Default.pp, R_DistRCH_Game23WOTSTW.O_R_DistRCH_Game23WOTSTW_THFC.adl, O_DistRCH.b}
            /\ O_DistRCH.ps{1} = O_SMDTUD_Default.pp{2}
            /\ O_SMDTUD_Default.pp{2} = O_THFC_Default.pp{2} 
            /\ O_SMDTUD_Default.b{2} = true
            /\ DistRCHil.O_DistRCHi.i{1} = k + 1
            /\ R_SMDTUDC_DistRCHil.O_R_SMDTUDC_DistRCHil.i{2} = k
-           /\ all is_chtype (map (fun (admpksig : adrs * msgWOTS * pkWOTS * sigWOTS) => admpksig.`1) O_MEFGCMA_WOTSTWES.qs{1})
-           /\ O_SMDTUD_Default.ts{2} = relcqsad_udi O_MEFGCMA_WOTSTWES.qs{1} k
+           /\ all is_chtype (map (fun (admpksig : adrs * msgWOTS * pkWOTS * sigWOTS) => admpksig.`1) O_MEUFGCMA_WOTSTWES.qs{1})
+           /\ O_SMDTUD_Default.ts{2} = relcqsad_udi O_MEUFGCMA_WOTSTWES.qs{1} k
            /\ all (fun (ad : adrs) => 
                        ad \in R_DistRCH_Game23WOTSTW.O_R_DistRCH_Game23WOTSTW_THFC.adl{2} 
-                       \/ ad \in reltqsad_udi O_MEFGCMA_WOTSTWES.qs{1} k) 
+                       \/ ad \in reltqsad_udi O_MEUFGCMA_WOTSTWES.qs{1} k) 
                        O_THFC_Default.tws{2}); last by auto.
     + proc.
-      seq 2 2 : (   ={glob O_MEFGCMA_WOTSTWES, O_THFC_Default.pp, R_DistRCH_Game23WOTSTW.O_R_DistRCH_Game23WOTSTW_THFC.adl, O_DistRCH.b, ad, m, chal}
+      seq 2 2 : (   ={glob O_MEUFGCMA_WOTSTWES, O_THFC_Default.pp, R_DistRCH_Game23WOTSTW.O_R_DistRCH_Game23WOTSTW_THFC.adl, O_DistRCH.b, ad, m, chal}
                  /\ is_chtype ad{1}
                  /\ O_DistRCH.ps{1} = O_SMDTUD_Default.pp{2}
                  /\ O_SMDTUD_Default.pp{2} = O_THFC_Default.pp{2}
                  /\ O_SMDTUD_Default.b{2} = true
                  /\ DistRCHil.O_DistRCHi.i{1} = k + 1
                  /\ R_SMDTUDC_DistRCHil.O_R_SMDTUDC_DistRCHil.i{2} = k
-                 /\ all is_chtype (map (fun (admpksig : adrs * msgWOTS * pkWOTS * sigWOTS) => admpksig.`1) O_MEFGCMA_WOTSTWES.qs{1})
-                 /\ O_SMDTUD_Default.ts{2} = relcqsad_udi (rcons O_MEFGCMA_WOTSTWES.qs{1} (ad{2}, m{2}, insubd pk{2}, insubd sig{2})) k
+                 /\ all is_chtype (map (fun (admpksig : adrs * msgWOTS * pkWOTS * sigWOTS) => admpksig.`1) O_MEUFGCMA_WOTSTWES.qs{1})
+                 /\ O_SMDTUD_Default.ts{2} = relcqsad_udi (rcons O_MEUFGCMA_WOTSTWES.qs{1} (ad{2}, m{2}, insubd pk{2}, insubd sig{2})) k
                  /\ all (fun (ad' : adrs) => 
                              ad' \in R_DistRCH_Game23WOTSTW.O_R_DistRCH_Game23WOTSTW_THFC.adl{2} 
-                             \/ ad' \in reltqsad_udi (rcons O_MEFGCMA_WOTSTWES.qs{1} (ad{2}, m{2}, insubd pk{2}, insubd sig{2})) k) 
+                             \/ ad' \in reltqsad_udi (rcons O_MEUFGCMA_WOTSTWES.qs{1} (ad{2}, m{2}, insubd pk{2}, insubd sig{2})) k) 
                              O_THFC_Default.tws{2}
                  /\ size chal{1} = len).
       - inline *; swap{1} 5 -2.
         wp => /=.
-        while (   ={glob O_MEFGCMA_WOTSTWES, O_THFC_Default.pp, R_DistRCH_Game23WOTSTW.O_R_DistRCH_Game23WOTSTW_THFC.adl, O_DistRCH.b, ad, m, ad0, m0, em0, chal0, chal'}
+        while (   ={glob O_MEUFGCMA_WOTSTWES, O_THFC_Default.pp, R_DistRCH_Game23WOTSTW.O_R_DistRCH_Game23WOTSTW_THFC.adl, O_DistRCH.b, ad, m, ad0, m0, em0, chal0, chal'}
                /\ ad0{1} = ad{1}
                /\ m0{1} = m{1}
                /\ em0{1} = encode_msgWOTS m0{1}
@@ -5956,11 +5956,11 @@ have ->:
                /\ O_SMDTUD_Default.b{2} = true
                /\ DistRCHil.O_DistRCHi.i{1} = k + 1
                /\ R_SMDTUDC_DistRCHil.O_R_SMDTUDC_DistRCHil.i{2} = k
-               /\ all is_chtype (map (fun (admpksig : adrs * msgWOTS * pkWOTS * sigWOTS) => admpksig.`1) O_MEFGCMA_WOTSTWES.qs{1})
-               /\ O_SMDTUD_Default.ts{2} = relcqsad_udi (rcons O_MEFGCMA_WOTSTWES.qs{1} (ad{2}, m{2}, insubd pk{2}, insubd sig{2})) k
+               /\ all is_chtype (map (fun (admpksig : adrs * msgWOTS * pkWOTS * sigWOTS) => admpksig.`1) O_MEUFGCMA_WOTSTWES.qs{1})
+               /\ O_SMDTUD_Default.ts{2} = relcqsad_udi (rcons O_MEUFGCMA_WOTSTWES.qs{1} (ad{2}, m{2}, insubd pk{2}, insubd sig{2})) k
                /\ all (fun (ad' : adrs) => 
                            ad' \in R_DistRCH_Game23WOTSTW.O_R_DistRCH_Game23WOTSTW_THFC.adl{2} 
-                           \/ ad' \in reltqsad_udi (rcons O_MEFGCMA_WOTSTWES.qs{1} (ad{2}, m{2}, insubd pk{2}, insubd sig{2})) k) 
+                           \/ ad' \in reltqsad_udi (rcons O_MEUFGCMA_WOTSTWES.qs{1} (ad{2}, m{2}, insubd pk{2}, insubd sig{2})) k) 
                            O_THFC_Default.tws{2}
                /\ size chal'{1} = len
                /\ 0 <= size chal0{1} <= len).
@@ -5979,7 +5979,7 @@ have ->:
                     /\ chal_ele0{2} = cf O_THFC_Default.pp{2} (set_chthidx ad0{2} (size chal0{2})) (R_SMDTUDC_DistRCHil.O_R_SMDTUDC_DistRCHil.i{2} + 1) (j0{2} - 1) (val (nth witness chal'{2} (size chal0{2})))
                     /\ all (fun (ad' : adrs) => 
                            ad' \in R_DistRCH_Game23WOTSTW.O_R_DistRCH_Game23WOTSTW_THFC.adl{2} 
-                           \/ ad' \in reltqsad_udi (rcons O_MEFGCMA_WOTSTWES.qs{1} (ad{2}, m{2}, insubd pk{2}, insubd sig{2})) k) 
+                           \/ ad' \in reltqsad_udi (rcons O_MEUFGCMA_WOTSTWES.qs{1} (ad{2}, m{2}, insubd pk{2}, insubd sig{2})) k) 
                            O_THFC_Default.tws{2}
                     /\ size chal'{2} = len
                     /\ 0 <= size chal0{2} < len
@@ -6001,7 +6001,7 @@ have ->:
           wp; skip => /> &2 adch qsch twssp eqlen_szcp ge0_szc0 lelen_szc0 ltlen_szc0 leem1k_j.
           by split => [| twsr jr]; [rewrite /cf ch0 1:ischtype_setchidx 3:valP //= valKd /# | smt(size_rcons)].
         wp => /=.
-        while (   ={glob O_MEFGCMA_WOTSTWES, O_THFC_Default.pp, R_DistRCH_Game23WOTSTW.O_R_DistRCH_Game23WOTSTW_THFC.adl, O_DistRCH.b, ad, m, ad0, m0, chal'}
+        while (   ={glob O_MEUFGCMA_WOTSTWES, O_THFC_Default.pp, R_DistRCH_Game23WOTSTW.O_R_DistRCH_Game23WOTSTW_THFC.adl, O_DistRCH.b, ad, m, ad0, m0, chal'}
                    /\ ad0{1} = ad{1}
                    /\ m0{1} = m{1}
                    /\ em0{2} = encode_msgWOTS m0{2}
@@ -6011,14 +6011,14 @@ have ->:
                    /\ O_SMDTUD_Default.b{2} = true
                    /\ DistRCHil.O_DistRCHi.i{1} = k + 1
                    /\ R_SMDTUDC_DistRCHil.O_R_SMDTUDC_DistRCHil.i{2} = k
-                   /\ all is_chtype (map (fun (admpksig : adrs * msgWOTS * pkWOTS * sigWOTS) => admpksig.`1) O_MEFGCMA_WOTSTWES.qs{1})
+                   /\ all is_chtype (map (fun (admpksig : adrs * msgWOTS * pkWOTS * sigWOTS) => admpksig.`1) O_MEUFGCMA_WOTSTWES.qs{1})
                    /\ O_SMDTUD_Default.ts{2} 
                       = 
-                      relcqsad_udi O_MEFGCMA_WOTSTWES.qs{1} k 
+                      relcqsad_udi O_MEUFGCMA_WOTSTWES.qs{1} k 
                       ++ relcqsad_udi_outer ad0{2} m0{2} k (size chal'{2})
                    /\ all (fun (ad' : adrs) => 
                                ad' \in R_DistRCH_Game23WOTSTW.O_R_DistRCH_Game23WOTSTW_THFC.adl{2} 
-                               \/ ad' \in reltqsad_udi (rcons O_MEFGCMA_WOTSTWES.qs{1} (ad{2}, m{2}, insubd pk{2}, insubd sig{2})) k) 
+                               \/ ad' \in reltqsad_udi (rcons O_MEUFGCMA_WOTSTWES.qs{1} (ad{2}, m{2}, insubd pk{2}, insubd sig{2})) k) 
                                O_THFC_Default.tws{2}
                    /\ 0 <= size chal'{1} <= len).
         * wp; sp => /=.
@@ -6115,9 +6115,9 @@ have ->:
   split; last by apply uniq_relcqsadudi => /#.
   rewrite andbC; split; first split => [| _].
   * by smt(relcqsadudi_rng).
-  * apply (IntOrder.ler_trans (size O_MEFGCMA_WOTSTWES.qs{2} * len)); first by smt(relcqsadudi_rng).
+  * apply (IntOrder.ler_trans (size O_MEUFGCMA_WOTSTWES.qs{2} * len)); first by smt(relcqsadudi_rng).
     by rewrite ler_pmul //; smt(ge2_len).
-  apply (djl_parts _ _ R_DistRCH_Game23WOTSTW.O_R_DistRCH_Game23WOTSTW_THFC.adl{2} (reltqsad_udi O_MEFGCMA_WOTSTWES.qs{2} k)) => //. 
+  apply (djl_parts _ _ R_DistRCH_Game23WOTSTW.O_R_DistRCH_Game23WOTSTW_THFC.adl{2} (reltqsad_udi O_MEUFGCMA_WOTSTWES.qs{2} k)) => //. 
   * by apply disj_relcqsadudi => /#.
   by apply disj_relcqsadudi_reltqsadudi => /#.
 have ->:
@@ -6183,14 +6183,14 @@ do 3! congr; rewrite eq_sym Pr[mu_split 0 <= R_SMDTUDC_DistRCH.O_R_SMDTUDC_DistR
   byequiv => //.
   proc; inline{1} 2; inline{1} 7; inline{2} 4.
   swap{1} 4 -3; swap{2} 4 -2. 
-  seq 10 6 : (   ={glob A, pp, R_DistRCH_Game23WOTSTW.O_R_DistRCH_Game23WOTSTW_THFC.adl, O_MEFGCMA_WOTSTWES.qs, O_SMDTUD_Default.ts, O_THFC_Default.tws}
+  seq 10 6 : (   ={glob A, pp, R_DistRCH_Game23WOTSTW.O_R_DistRCH_Game23WOTSTW_THFC.adl, O_MEUFGCMA_WOTSTWES.qs, O_SMDTUD_Default.ts, O_THFC_Default.tws}
                /\ i{1} = R_SMDTUDC_DistRCH.O_R_SMDTUDC_DistRCH.i{2}); last by wp => /=; sim.
   inline *.
-  call (:   ={R_DistRCH_Game23WOTSTW.O_R_DistRCH_Game23WOTSTW_THFC.adl, O_MEFGCMA_WOTSTWES.qs, O_SMDTUD_Default.b, O_SMDTUD_Default.pp, O_SMDTUD_Default.ts, O_THFC_Default.tws, O_THFC_Default.pp}
+  call (:   ={R_DistRCH_Game23WOTSTW.O_R_DistRCH_Game23WOTSTW_THFC.adl, O_MEUFGCMA_WOTSTWES.qs, O_SMDTUD_Default.b, O_SMDTUD_Default.pp, O_SMDTUD_Default.ts, O_THFC_Default.tws, O_THFC_Default.pp}
          /\ R_SMDTUDC_DistRCHil.O_R_SMDTUDC_DistRCHil.i{1} = R_SMDTUDC_DistRCH.O_R_SMDTUDC_DistRCH.i{2}).
   - proc.
     inline *.
-    seq 7 7 : (   ={m, em0, chal', ad0, ad, R_DistRCH_Game23WOTSTW.O_R_DistRCH_Game23WOTSTW_THFC.adl, O_MEFGCMA_WOTSTWES.qs, O_SMDTUD_Default.b, O_SMDTUD_Default.pp, O_SMDTUD_Default.ts, O_THFC_Default.tws, O_THFC_Default.pp}
+    seq 7 7 : (   ={m, em0, chal', ad0, ad, R_DistRCH_Game23WOTSTW.O_R_DistRCH_Game23WOTSTW_THFC.adl, O_MEUFGCMA_WOTSTWES.qs, O_SMDTUD_Default.b, O_SMDTUD_Default.pp, O_SMDTUD_Default.ts, O_THFC_Default.tws, O_THFC_Default.pp}
                /\ is_chtype ad{1}
                /\ ad0{1} = ad{1}
                /\ R_SMDTUDC_DistRCHil.O_R_SMDTUDC_DistRCHil.i{1} = R_SMDTUDC_DistRCH.O_R_SMDTUDC_DistRCH.i{2}); last by sim.
@@ -6216,14 +6216,14 @@ rewrite (indbigsplit (w - 2)); first by smt(val_w).
 byequiv => //.
 proc; inline{1} 2; inline{1} 7; inline{2} 4.
 swap{1} 4 -3; swap{2} 4 -2.
-seq 10 6 : (   ={glob A, pp, R_DistRCH_Game23WOTSTW.O_R_DistRCH_Game23WOTSTW_THFC.adl, O_MEFGCMA_WOTSTWES.qs, O_SMDTUD_Default.ts, O_THFC_Default.tws}
+seq 10 6 : (   ={glob A, pp, R_DistRCH_Game23WOTSTW.O_R_DistRCH_Game23WOTSTW_THFC.adl, O_MEUFGCMA_WOTSTWES.qs, O_SMDTUD_Default.ts, O_THFC_Default.tws}
                /\ i{1} = R_SMDTUDC_DistRCH.O_R_SMDTUDC_DistRCH.i{2}); last by wp => /=; sim.
 inline *.
-call (:   ={R_DistRCH_Game23WOTSTW.O_R_DistRCH_Game23WOTSTW_THFC.adl, O_MEFGCMA_WOTSTWES.qs, O_SMDTUD_Default.b, O_SMDTUD_Default.pp, O_SMDTUD_Default.ts, O_THFC_Default.tws, O_THFC_Default.pp}
+call (:   ={R_DistRCH_Game23WOTSTW.O_R_DistRCH_Game23WOTSTW_THFC.adl, O_MEUFGCMA_WOTSTWES.qs, O_SMDTUD_Default.b, O_SMDTUD_Default.pp, O_SMDTUD_Default.ts, O_THFC_Default.tws, O_THFC_Default.pp}
          /\ R_SMDTUDC_DistRCHil.O_R_SMDTUDC_DistRCHil.i{1} = R_SMDTUDC_DistRCH.O_R_SMDTUDC_DistRCH.i{2}).
 + proc.
   inline *.
-  seq 7 7 : (   ={m, em0, chal', ad0, ad, R_DistRCH_Game23WOTSTW.O_R_DistRCH_Game23WOTSTW_THFC.adl, O_MEFGCMA_WOTSTWES.qs, O_SMDTUD_Default.b, O_SMDTUD_Default.pp, O_SMDTUD_Default.ts, O_THFC_Default.tws, O_THFC_Default.pp}
+  seq 7 7 : (   ={m, em0, chal', ad0, ad, R_DistRCH_Game23WOTSTW.O_R_DistRCH_Game23WOTSTW_THFC.adl, O_MEUFGCMA_WOTSTWES.qs, O_SMDTUD_Default.b, O_SMDTUD_Default.pp, O_SMDTUD_Default.ts, O_THFC_Default.tws, O_THFC_Default.pp}
              /\ is_chtype ad{1}
              /\ ad0{1} = ad{1} 
              /\ R_SMDTUDC_DistRCHil.O_R_SMDTUDC_DistRCHil.i{1} = R_SMDTUDC_DistRCH.O_R_SMDTUDC_DistRCH.i{2}); last by sim.
@@ -6260,9 +6260,9 @@ have ->:
   Pr[Game3_WOTSTWES.main() @ &m : res] = Pr[Game3_WOTSTWES_Hchwcoll.main() @ &m : res].
 + byequiv => //. 
   proc; inline *.
-  seq 12 11 : (={glob O_THFC_Default, O_MEFGCMA_WOTSTWES.qs, ps, i, m', sig'}); last first.
-  - by wp; sim : (={i, m, m', O_MEFGCMA_WOTSTWES.qs, O_THFC_Default.tws} /\ pkWOTS0{1} = pkWOTS{2} /\ pkWOTS1{1} = pkWOTS0{2}).
-  do 2! call (: ={glob O_THFC_Default, O_MEFGCMA_WOTSTWES.qs, O_MEFGCMA_WOTSTWES.ps}); first 2 by proc; inline *; sim.
+  seq 12 11 : (={glob O_THFC_Default, O_MEUFGCMA_WOTSTWES.qs, ps, i, m', sig'}); last first.
+  - by wp; sim : (={i, m, m', O_MEUFGCMA_WOTSTWES.qs, O_THFC_Default.tws} /\ pkWOTS0{1} = pkWOTS{2} /\ pkWOTS1{1} = pkWOTS0{2}).
+  do 2! call (: ={glob O_THFC_Default, O_MEUFGCMA_WOTSTWES.qs, O_MEUFGCMA_WOTSTWES.ps}); first 2 by proc; inline *; sim.
    by auto.
 rewrite Pr[mu_split Game3_WOTSTWES_Hchwcoll.hchwcoll].
 have -> /#: 
@@ -6271,7 +6271,7 @@ have -> /#:
   Pr[Game4_WOTSTWES.main() @ &m : res].
 byequiv => //.
 proc; inline *. wp.
-by wp; sim :  (={i, ps, pkWOTS0, pkWOTS, ad, m, m', sig, sig', O_MEFGCMA_WOTSTWES.qs, O_THFC_Default.tws}).
+by wp; sim :  (={i, ps, pkWOTS0, pkWOTS, ad, m, m', sig, sig', O_MEUFGCMA_WOTSTWES.qs, O_THFC_Default.tws}).
 qed.
 
 (* Fourth step: Reduce SM-DT-TCR-C of f to distinguishing between Game3_WOTSTWES and Game4_WOTSTWES *)
@@ -6287,12 +6287,12 @@ swap{2} 13 -11.
 wp => /=.
 seq 9 12 : (   ={glob A, ps}
             /\ pp{2} = ps{2}
-            /\ O_MEFGCMA_WOTSTWES.ps{1} = ps{1}
+            /\ O_MEUFGCMA_WOTSTWES.ps{1} = ps{1}
             /\ O_THFC_Default.pp{1} = ps{1}
             /\ O_SMDTTCR_Default.pp{2} = ps{2}
             /\ O_THFC_Default.pp{2} = ps{2}
-            /\ O_MEFGCMA_WOTSTWES.qs{1} = []
-            /\ O_MEFGCMA_WOTSTWES.qs{2} = []
+            /\ O_MEUFGCMA_WOTSTWES.qs{1} = []
+            /\ O_MEUFGCMA_WOTSTWES.qs{2} = []
             /\ R_SMDTTCRC_Game34WOTSTWES.O_R_SMDTTCRC_Game34WOTSTWES.xll{2} = []
             /\ O_THFC_Default.tws{1} = []
             /\ O_SMDTTCR_Default.ts{2} = []
@@ -6319,28 +6319,28 @@ pose sigvals (qs : (adrs * msgWOTS * pkWOTS * sigWOTS) list) (xll : dgstblock li
                if em_ele <> 0
                then cf ps (set_chthidx ad j) (em_ele - 1) 1 (val (nth witness xl j))
                else nth witness xl j) (range 0 i)) (zip qs xll).
-seq 1 1 : (    ={glob A, glob O_THFC_Default, O_MEFGCMA_WOTSTWES.qs, ps}
+seq 1 1 : (    ={glob A, glob O_THFC_Default, O_MEUFGCMA_WOTSTWES.qs, ps}
             /\ pp{2} = ps{2}
-            /\ O_MEFGCMA_WOTSTWES.ps{1} = ps{1}
+            /\ O_MEUFGCMA_WOTSTWES.ps{1} = ps{1}
             /\ O_THFC_Default.pp{1} = ps{1}
             /\ O_SMDTTCR_Default.pp{2} = ps{2}
             /\ O_THFC_Default.pp{2} = ps{2}
-            /\ size O_MEFGCMA_WOTSTWES.qs{1} = size R_SMDTTCRC_Game34WOTSTWES.O_R_SMDTTCRC_Game34WOTSTWES.xll{2}
-            /\ all is_chtype (map (fun (admpksig : adrs * msgWOTS * pkWOTS * sigWOTS) => admpksig.`1) O_MEFGCMA_WOTSTWES.qs{1})
-            /\ pkvals O_MEFGCMA_WOTSTWES.qs{1} O_MEFGCMA_WOTSTWES.ps{1} len
-            /\ sigvals O_MEFGCMA_WOTSTWES.qs{1} R_SMDTTCRC_Game34WOTSTWES.O_R_SMDTTCRC_Game34WOTSTWES.xll{2} O_MEFGCMA_WOTSTWES.ps{1} len
-            /\ unzip1 O_SMDTTCR_Default.ts{2} = relcqsad_tcr O_MEFGCMA_WOTSTWES.qs{1}
-            /\ unzip2 O_SMDTTCR_Default.ts{2} = relcqsdg_tcr O_MEFGCMA_WOTSTWES.qs{1} R_SMDTTCRC_Game34WOTSTWES.O_R_SMDTTCRC_Game34WOTSTWES.xll{2} O_MEFGCMA_WOTSTWES.ps{1}).
-+ call (:   ={glob O_THFC_Default, O_MEFGCMA_WOTSTWES.qs}
-         /\ O_MEFGCMA_WOTSTWES.ps{1} = O_THFC_Default.pp{1}
+            /\ size O_MEUFGCMA_WOTSTWES.qs{1} = size R_SMDTTCRC_Game34WOTSTWES.O_R_SMDTTCRC_Game34WOTSTWES.xll{2}
+            /\ all is_chtype (map (fun (admpksig : adrs * msgWOTS * pkWOTS * sigWOTS) => admpksig.`1) O_MEUFGCMA_WOTSTWES.qs{1})
+            /\ pkvals O_MEUFGCMA_WOTSTWES.qs{1} O_MEUFGCMA_WOTSTWES.ps{1} len
+            /\ sigvals O_MEUFGCMA_WOTSTWES.qs{1} R_SMDTTCRC_Game34WOTSTWES.O_R_SMDTTCRC_Game34WOTSTWES.xll{2} O_MEUFGCMA_WOTSTWES.ps{1} len
+            /\ unzip1 O_SMDTTCR_Default.ts{2} = relcqsad_tcr O_MEUFGCMA_WOTSTWES.qs{1}
+            /\ unzip2 O_SMDTTCR_Default.ts{2} = relcqsdg_tcr O_MEUFGCMA_WOTSTWES.qs{1} R_SMDTTCRC_Game34WOTSTWES.O_R_SMDTTCRC_Game34WOTSTWES.xll{2} O_MEUFGCMA_WOTSTWES.ps{1}).
++ call (:   ={glob O_THFC_Default, O_MEUFGCMA_WOTSTWES.qs}
+         /\ O_MEUFGCMA_WOTSTWES.ps{1} = O_THFC_Default.pp{1}
          /\ O_THFC_Default.pp{1} = O_THFC_Default.pp{2}
          /\ O_THFC_Default.pp{2} = O_SMDTTCR_Default.pp{2}
-         /\ size O_MEFGCMA_WOTSTWES.qs{1} = size R_SMDTTCRC_Game34WOTSTWES.O_R_SMDTTCRC_Game34WOTSTWES.xll{2}
-         /\ all is_chtype (map (fun (admpksig : adrs * msgWOTS * pkWOTS * sigWOTS) => admpksig.`1) O_MEFGCMA_WOTSTWES.qs{1})
-         /\ pkvals O_MEFGCMA_WOTSTWES.qs{1} O_MEFGCMA_WOTSTWES.ps{1} len
-         /\ sigvals O_MEFGCMA_WOTSTWES.qs{1} R_SMDTTCRC_Game34WOTSTWES.O_R_SMDTTCRC_Game34WOTSTWES.xll{2} O_MEFGCMA_WOTSTWES.ps{1} len
-         /\ unzip1 O_SMDTTCR_Default.ts{2} = relcqsad_tcr O_MEFGCMA_WOTSTWES.qs{1}
-         /\ unzip2 O_SMDTTCR_Default.ts{2} = relcqsdg_tcr O_MEFGCMA_WOTSTWES.qs{1} R_SMDTTCRC_Game34WOTSTWES.O_R_SMDTTCRC_Game34WOTSTWES.xll{2} O_MEFGCMA_WOTSTWES.ps{1}); last by auto.
+         /\ size O_MEUFGCMA_WOTSTWES.qs{1} = size R_SMDTTCRC_Game34WOTSTWES.O_R_SMDTTCRC_Game34WOTSTWES.xll{2}
+         /\ all is_chtype (map (fun (admpksig : adrs * msgWOTS * pkWOTS * sigWOTS) => admpksig.`1) O_MEUFGCMA_WOTSTWES.qs{1})
+         /\ pkvals O_MEUFGCMA_WOTSTWES.qs{1} O_MEUFGCMA_WOTSTWES.ps{1} len
+         /\ sigvals O_MEUFGCMA_WOTSTWES.qs{1} R_SMDTTCRC_Game34WOTSTWES.O_R_SMDTTCRC_Game34WOTSTWES.xll{2} O_MEUFGCMA_WOTSTWES.ps{1} len
+         /\ unzip1 O_SMDTTCR_Default.ts{2} = relcqsad_tcr O_MEUFGCMA_WOTSTWES.qs{1}
+         /\ unzip2 O_SMDTTCR_Default.ts{2} = relcqsdg_tcr O_MEUFGCMA_WOTSTWES.qs{1} R_SMDTTCRC_Game34WOTSTWES.O_R_SMDTTCRC_Game34WOTSTWES.xll{2} O_MEUFGCMA_WOTSTWES.ps{1}); last by auto.
   - proc; inline * => //.
     seq 6 5 : (   #pre
                /\ ={ad, pk, em}
@@ -6357,7 +6357,7 @@ seq 1 1 : (    ={glob A, glob O_THFC_Default, O_MEFGCMA_WOTSTWES.qs, ps}
                      nth witness sig{1} i 
                      = 
                      if BaseW.val em{1}.[i] <> 0
-                     then cf O_MEFGCMA_WOTSTWES.ps{1} (set_chthidx ad{1} i) (BaseW.val em{1}.[i] - 1) 1 (val (nth witness sk{1} i))
+                     then cf O_MEUFGCMA_WOTSTWES.ps{1} (set_chthidx ad{1} i) (BaseW.val em{1}.[i] - 1) 1 (val (nth witness sk{1} i))
                      else nth witness sk{1} i)).
     * wp => /=.
       while{1} (   is_chtype ad{1}
@@ -6366,7 +6366,7 @@ seq 1 1 : (    ={glob A, glob O_THFC_Default, O_MEFGCMA_WOTSTWES.qs, ps}
                       nth witness sig{1} i
                       = 
                       if BaseW.val em{1}.[i] <> 0
-                      then cf O_MEFGCMA_WOTSTWES.ps{1} (set_chthidx ad{1} i) (BaseW.val em{1}.[i] - 1) 1 (val (nth witness sk{1} i))
+                      then cf O_MEUFGCMA_WOTSTWES.ps{1} (set_chthidx ad{1} i) (BaseW.val em{1}.[i] - 1) 1 (val (nth witness sk{1} i))
                       else nth witness sk{1} i))
                (len - size sig{1}).
       + move=> _ z; wp; skip => /> &1 adch _ valsig ltlen_szsig.
@@ -6381,19 +6381,19 @@ seq 1 1 : (    ={glob A, glob O_THFC_Default, O_MEFGCMA_WOTSTWES.qs, ps}
         by rewrite (: i = size sig{1}) 1:/# /= neq0_em.
       wp; rnd; wp; skip => /> *; split; smt(ge2_len ChainingAddress.valP).
     wp => //=.
-    while (   ={glob O_THFC_Default, ad, m, pk, em, O_MEFGCMA_WOTSTWES.qs} 
-           /\ O_MEFGCMA_WOTSTWES.ps{1} = O_THFC_Default.pp{1}
+    while (   ={glob O_THFC_Default, ad, m, pk, em, O_MEUFGCMA_WOTSTWES.qs} 
+           /\ O_MEUFGCMA_WOTSTWES.ps{1} = O_THFC_Default.pp{1}
            /\ O_THFC_Default.pp{1} = O_THFC_Default.pp{2} 
            /\ O_THFC_Default.pp{2} = O_SMDTTCR_Default.pp{2}
-           /\ size O_MEFGCMA_WOTSTWES.qs{1} = size R_SMDTTCRC_Game34WOTSTWES.O_R_SMDTTCRC_Game34WOTSTWES.xll{2}
+           /\ size O_MEUFGCMA_WOTSTWES.qs{1} = size R_SMDTTCRC_Game34WOTSTWES.O_R_SMDTTCRC_Game34WOTSTWES.xll{2}
            /\ unzip1 O_SMDTTCR_Default.ts{2} 
               = 
-              relcqsad_tcr O_MEFGCMA_WOTSTWES.qs{1} 
+              relcqsad_tcr O_MEUFGCMA_WOTSTWES.qs{1} 
               ++ relcqsad_tcr_outer ad{2} m{2} (size pk{2})
            /\ unzip2 O_SMDTTCR_Default.ts{2} 
               = 
-              relcqsdg_tcr O_MEFGCMA_WOTSTWES.qs{1} R_SMDTTCRC_Game34WOTSTWES.O_R_SMDTTCRC_Game34WOTSTWES.xll{2} O_MEFGCMA_WOTSTWES.ps{1} 
-              ++ relcqsdg_tcr_outer O_MEFGCMA_WOTSTWES.ps{1} ad{2} m{2} (insubd sig{1}) xl{2} (size pk{2})
+              relcqsdg_tcr O_MEUFGCMA_WOTSTWES.qs{1} R_SMDTTCRC_Game34WOTSTWES.O_R_SMDTTCRC_Game34WOTSTWES.xll{2} O_MEUFGCMA_WOTSTWES.ps{1} 
+              ++ relcqsdg_tcr_outer O_MEUFGCMA_WOTSTWES.ps{1} ad{2} m{2} (insubd sig{1}) xl{2} (size pk{2})
            /\ is_chtype ad{1} 
            /\ em{1} = encode_msgWOTS m{1} 
            /\ em{2} = encode_msgWOTS m{2} 
@@ -6409,30 +6409,30 @@ seq 1 1 : (    ={glob A, glob O_THFC_Default, O_MEFGCMA_WOTSTWES.qs, ps}
                 nth witness sig{1} i 
                 =
                 if (BaseW.val em{1}.[i]) <> 0 
-                then cf O_MEFGCMA_WOTSTWES.ps{1} (set_chthidx ad{1} i)((BaseW.val em{1}.[i]) - 1) 1 (val (nth witness sk{1} i))
+                then cf O_MEUFGCMA_WOTSTWES.ps{1} (set_chthidx ad{1} i)((BaseW.val em{1}.[i]) - 1) 1 (val (nth witness sk{1} i))
                 else nth witness sk{1} i)
            /\ (forall (i : int), 0 <= i < size pk{1} =>
                 nth witness pk{1} i 
                 =
-                cf O_MEFGCMA_WOTSTWES.ps{1} (set_chthidx ad{1} i) (BaseW.val em{1}.[i]) (w - 1 - BaseW.val em{1}.[i]) (val (nth witness sig{1} i)))
+                cf O_MEUFGCMA_WOTSTWES.ps{1} (set_chthidx ad{1} i) (BaseW.val em{1}.[i]) (w - 1 - BaseW.val em{1}.[i]) (val (nth witness sig{1} i)))
            /\ (forall (i : int), 0 <= i && i < size sig{2} =>
                  nth witness sig{1} i = nth witness sig{2} i)).
     * wp => /=.
-      while{2} (   ={glob O_THFC_Default, ad, m, pk, em, O_MEFGCMA_WOTSTWES.qs} 
-                /\ O_MEFGCMA_WOTSTWES.ps{1} = O_THFC_Default.pp{1} 
+      while{2} (   ={glob O_THFC_Default, ad, m, pk, em, O_MEUFGCMA_WOTSTWES.qs} 
+                /\ O_MEUFGCMA_WOTSTWES.ps{1} = O_THFC_Default.pp{1} 
                 /\ O_THFC_Default.pp{1} = O_THFC_Default.pp{2} 
                 /\ O_THFC_Default.pp{2} = O_SMDTTCR_Default.pp{2}
-                /\ size O_MEFGCMA_WOTSTWES.qs{1} = size R_SMDTTCRC_Game34WOTSTWES.O_R_SMDTTCRC_Game34WOTSTWES.xll{2}
+                /\ size O_MEUFGCMA_WOTSTWES.qs{1} = size R_SMDTTCRC_Game34WOTSTWES.O_R_SMDTTCRC_Game34WOTSTWES.xll{2}
                 /\ unzip1 O_SMDTTCR_Default.ts{2} 
                    = 
-                   relcqsad_tcr O_MEFGCMA_WOTSTWES.qs{1} 
+                   relcqsad_tcr O_MEUFGCMA_WOTSTWES.qs{1} 
                    ++ relcqsad_tcr_outer ad{2} m{2} (size pk{2})
                    ++ relcqsad_tcr_inner (set_chthidx ad{2} (size pk{2})) em_ele{2} j{2}
                 /\ unzip2 O_SMDTTCR_Default.ts{2} 
                    = 
-                   relcqsdg_tcr O_MEFGCMA_WOTSTWES.qs{1} R_SMDTTCRC_Game34WOTSTWES.O_R_SMDTTCRC_Game34WOTSTWES.xll{2} O_MEFGCMA_WOTSTWES.ps{1} 
-                   ++ relcqsdg_tcr_outer O_MEFGCMA_WOTSTWES.ps{1} ad{2} m{2} (insubd sig{1}) xl{2} (size pk{2})
-                   ++ relcqsdg_tcr_inner O_MEFGCMA_WOTSTWES.ps{1} (set_chthidx ad{2} (size pk{2})) em_ele{2} sig_ele{2} x{2} j{2}
+                   relcqsdg_tcr O_MEUFGCMA_WOTSTWES.qs{1} R_SMDTTCRC_Game34WOTSTWES.O_R_SMDTTCRC_Game34WOTSTWES.xll{2} O_MEUFGCMA_WOTSTWES.ps{1} 
+                   ++ relcqsdg_tcr_outer O_MEUFGCMA_WOTSTWES.ps{1} ad{2} m{2} (insubd sig{1}) xl{2} (size pk{2})
+                   ++ relcqsdg_tcr_inner O_MEUFGCMA_WOTSTWES.ps{1} (set_chthidx ad{2} (size pk{2})) em_ele{2} sig_ele{2} x{2} j{2}
                 /\ is_chtype ad{1} 
                 /\ em{1} = encode_msgWOTS m{1} 
                 /\ em{2} = encode_msgWOTS m{2} 
@@ -6448,12 +6448,12 @@ seq 1 1 : (    ={glob A, glob O_THFC_Default, O_MEFGCMA_WOTSTWES.qs, ps}
                      nth witness sig{1} i 
                      =
                      if (BaseW.val em{1}.[i]) <> 0 
-                     then cf O_MEFGCMA_WOTSTWES.ps{1} (set_chthidx ad{1} i)((BaseW.val em{1}.[i]) - 1) 1 (val (nth witness sk{1} i))
+                     then cf O_MEUFGCMA_WOTSTWES.ps{1} (set_chthidx ad{1} i)((BaseW.val em{1}.[i]) - 1) 1 (val (nth witness sk{1} i))
                      else nth witness sk{1} i)
                 /\ (forall (i : int), 0 <= i < size pk{1} =>
                       nth witness pk{1} i 
                       =
-                      cf O_MEFGCMA_WOTSTWES.ps{1} (set_chthidx ad{1} i) (BaseW.val em{1}.[i]) (w - 1 - BaseW.val em{1}.[i]) (val (nth witness sig{1} i)))  
+                      cf O_MEUFGCMA_WOTSTWES.ps{1} (set_chthidx ad{1} i) (BaseW.val em{1}.[i]) (w - 1 - BaseW.val em{1}.[i]) (val (nth witness sig{1} i)))  
                 /\ (forall (i : int), 0 <= i && i < size sig{2} =>
                       nth witness sig{1} i = nth witness sig{2} i)
                 /\ em_ele{2} = BaseW.val em{2}.[size pk{2}]
@@ -6543,7 +6543,7 @@ seq 1 1 : (   #pre
            /\ ={m', sig'}
            /\ i{1} = i0{2}).
 + by call(: true); skip.
-case (0 <= i{1} < size O_MEFGCMA_WOTSTWES.qs{1}); last first.
+case (0 <= i{1} < size O_MEUFGCMA_WOTSTWES.qs{1}); last first.
 + conseq (: _ ==> true) => [/#| ]. 
   while{1} (true) (len - size pkWOTS0{1}); first by auto; smt(size_rcons).
   by wp; skip => /> /#.
@@ -6574,74 +6574,74 @@ split; first by smt(uniq_relcqsadtcr allP all_map).
 rewrite andbA; split; last by rewrite rcqsad &(disj_relcqsadtcr).
 pose i := find_chwcollidx _ _ _ _ _ _.
 pose j := find_collidx_l _ _ _ _ _ _.
-pose k := find_collidx_r ps{1} (set_chthidx (nth witness O_MEFGCMA_WOTSTWES.qs{1} i0{1}).`1 i)
-           (BaseW.val (encode_msgWOTS (nth witness O_MEFGCMA_WOTSTWES.qs{1} i0{1}).`2).[i])
+pose k := find_collidx_r ps{1} (set_chthidx (nth witness O_MEUFGCMA_WOTSTWES.qs{1} i0{1}).`1 i)
+           (BaseW.val (encode_msgWOTS (nth witness O_MEUFGCMA_WOTSTWES.qs{1} i0{1}).`2).[i])
            (BaseW.val (encode_msgWOTS m'{1}).[i])
-           (val (nth witness (val (nth witness O_MEFGCMA_WOTSTWES.qs{1} i0{1}).`4) i))
+           (val (nth witness (val (nth witness O_MEUFGCMA_WOTSTWES.qs{1} i0{1}).`4) i))
            (val (nth witness (val sig'{1}) i)).
 have rng_i: 0 <= i < len by apply hchwcoll_findchrng.
-move/allP: (qsch) => qsch'; move: (qsch' ((nth witness O_MEFGCMA_WOTSTWES.qs{1} i0{1}).`1) _) => //.
-+ by rewrite mapP; exists (nth witness O_MEFGCMA_WOTSTWES.qs{1} i0{1}); rewrite mem_nth.
+move/allP: (qsch) => qsch'; move: (qsch' ((nth witness O_MEUFGCMA_WOTSTWES.qs{1} i0{1}).`1) _) => //.
++ by rewrite mapP; exists (nth witness O_MEUFGCMA_WOTSTWES.qs{1} i0{1}); rewrite mem_nth.
 move => adch_i0.
 have eq_cf : 
-  cf ps{1} (set_chthidx (nth witness O_MEFGCMA_WOTSTWES.qs{1} i0{1}).`1 i)
-     (BaseW.val (encode_msgWOTS (nth witness O_MEFGCMA_WOTSTWES.qs{1} i0{1}).`2).[i])
-     (w - 1 - BaseW.val (encode_msgWOTS (nth witness O_MEFGCMA_WOTSTWES.qs{1} i0{1}).`2).[i])
-     (val (nth witness (val (nth witness O_MEFGCMA_WOTSTWES.qs{1} i0{1}).`4) i)) =
-  cf ps{1} (set_chthidx (nth witness O_MEFGCMA_WOTSTWES.qs{1} i0{1}).`1 i)
+  cf ps{1} (set_chthidx (nth witness O_MEUFGCMA_WOTSTWES.qs{1} i0{1}).`1 i)
+     (BaseW.val (encode_msgWOTS (nth witness O_MEUFGCMA_WOTSTWES.qs{1} i0{1}).`2).[i])
+     (w - 1 - BaseW.val (encode_msgWOTS (nth witness O_MEUFGCMA_WOTSTWES.qs{1} i0{1}).`2).[i])
+     (val (nth witness (val (nth witness O_MEUFGCMA_WOTSTWES.qs{1} i0{1}).`4) i)) =
+  cf ps{1} (set_chthidx (nth witness O_MEUFGCMA_WOTSTWES.qs{1} i0{1}).`1 i)
      (BaseW.val (encode_msgWOTS m'{1}).[i])
      (w - 1 - BaseW.val (encode_msgWOTS m'{1}).[i]) (val (nth witness (val sig'{1}) i)).
 + move: (pkpval i _); first by smt().
   rewrite insubdK // => <-.
   rewrite /pkvals allP /= in pkvs.
-  move: (pkvs (nth witness O_MEFGCMA_WOTSTWES.qs{1} i0{1}) _); first by rewrite mem_nth => /#.
+  move: (pkvs (nth witness O_MEUFGCMA_WOTSTWES.qs{1} i0{1}) _); first by rewrite mem_nth => /#.
   move/allP => /= h; move: (h i _); first by rewrite mem_range.
   by move => <-; rewrite -eqins_pk insubdK 1:/#.
 move/hchwcoll_hcoll /(_ _ _): (eq_cf) => // hcoll.
 move/hchwcoll_findlcollrng /(_ _ _): (eq_cf) => //; rewrite -/j -/i => rng_j.
 move/(nth_find witness): (hchwcoll); rewrite nth_range //= -/i; elim => ltem_emp neq_nthsig.
-have neq0_em: BaseW.val (encode_msgWOTS (nth witness O_MEFGCMA_WOTSTWES.qs{1} i0{1}).`2).[i] <> 0 by smt(BaseW.valP).
+have neq0_em: BaseW.val (encode_msgWOTS (nth witness O_MEUFGCMA_WOTSTWES.qs{1} i0{1}).`2).[i] <> 0 by smt(BaseW.valP).
 have ->:
-  (nth witness O_SMDTTCR_Default.ts{1} (qsdgtcr_idx O_MEFGCMA_WOTSTWES.qs{1} R_SMDTTCRC_Game34WOTSTWES.O_R_SMDTTCRC_Game34WOTSTWES.xll{1} ps{1} i0{1} i (j + 1))).`2
+  (nth witness O_SMDTTCR_Default.ts{1} (qsdgtcr_idx O_MEUFGCMA_WOTSTWES.qs{1} R_SMDTTCRC_Game34WOTSTWES.O_R_SMDTTCRC_Game34WOTSTWES.xll{1} ps{1} i0{1} i (j + 1))).`2
   =
-  nth witness (unzip2 O_SMDTTCR_Default.ts{1}) (qsdgtcr_idx O_MEFGCMA_WOTSTWES.qs{1} R_SMDTTCRC_Game34WOTSTWES.O_R_SMDTTCRC_Game34WOTSTWES.xll{1} ps{1} i0{1} i (j + 1)).
+  nth witness (unzip2 O_SMDTTCR_Default.ts{1}) (qsdgtcr_idx O_MEUFGCMA_WOTSTWES.qs{1} R_SMDTTCRC_Game34WOTSTWES.O_R_SMDTTCRC_Game34WOTSTWES.xll{1} ps{1} i0{1} i (j + 1)).
 + rewrite (nth_map witness witness) //.
   rewrite (: size O_SMDTTCR_Default.ts{1} = size (unzip2 O_SMDTTCR_Default.ts{1})) 1:size_map //. 
   by rewrite rcqsdg qsdgtcridx_rng // neq0_em /#.
 have ->:
   nth witness (unzip2 O_SMDTTCR_Default.ts{1}) 
-              (qsdgtcr_idx O_MEFGCMA_WOTSTWES.qs{1} R_SMDTTCRC_Game34WOTSTWES.O_R_SMDTTCRC_Game34WOTSTWES.xll{1} ps{1} i0{1} i (j + 1))
+              (qsdgtcr_idx O_MEUFGCMA_WOTSTWES.qs{1} R_SMDTTCRC_Game34WOTSTWES.O_R_SMDTTCRC_Game34WOTSTWES.xll{1} ps{1} i0{1} i (j + 1))
   =
-  val (extr_coll_l ps{1} (set_chthidx (nth witness O_MEFGCMA_WOTSTWES.qs{1} i0{1}).`1 i)
-              (BaseW.val (encode_msgWOTS (nth witness O_MEFGCMA_WOTSTWES.qs{1} i0{1}).`2).[i])
+  val (extr_coll_l ps{1} (set_chthidx (nth witness O_MEUFGCMA_WOTSTWES.qs{1} i0{1}).`1 i)
+              (BaseW.val (encode_msgWOTS (nth witness O_MEUFGCMA_WOTSTWES.qs{1} i0{1}).`2).[i])
               (BaseW.val (encode_msgWOTS m'{1}).[i])
-              (val (nth witness (val (nth witness O_MEFGCMA_WOTSTWES.qs{1} i0{1}).`4) i))
+              (val (nth witness (val (nth witness O_MEUFGCMA_WOTSTWES.qs{1} i0{1}).`4) i))
               (val (nth witness (val sig'{1}) i))).
 + rewrite rcqsdg nth_relcqsdgtcr_qsdgtcridx // 1:/# neq0_em /= /extr_coll_l -/cf -/j /=. 
   rewrite (Ring.IntID.addrC j 1) /cf ch_comp 1:ischtype_setchidx 3:valP //=; first 3 smt(BaseW.valP).
   congr; rewrite /sigvals allP /= in sigvs.
   move: (sigvs (nth (witness, witness) 
-               (zip O_MEFGCMA_WOTSTWES.qs{1} R_SMDTTCRC_Game34WOTSTWES.O_R_SMDTTCRC_Game34WOTSTWES.xll{1}) i0{1}) _). 
+               (zip O_MEUFGCMA_WOTSTWES.qs{1} R_SMDTTCRC_Game34WOTSTWES.O_R_SMDTTCRC_Game34WOTSTWES.xll{1}) i0{1}) _). 
   - by rewrite mem_nth; smt(size_zip).
   move/allP => /= h; move: (h i _); first by rewrite mem_range.
   by rewrite ?nth_zip // neq0_em /= => ->.
 have ->: 
   (nth witness O_SMDTTCR_Default.ts{1}
-     (qsdgtcr_idx O_MEFGCMA_WOTSTWES.qs{1} R_SMDTTCRC_Game34WOTSTWES.O_R_SMDTTCRC_Game34WOTSTWES.xll{1} ps{1} i0{1} i (j + 1))).`1
+     (qsdgtcr_idx O_MEUFGCMA_WOTSTWES.qs{1} R_SMDTTCRC_Game34WOTSTWES.O_R_SMDTTCRC_Game34WOTSTWES.xll{1} ps{1} i0{1} i (j + 1))).`1
   =
-  nth witness (unzip1 O_SMDTTCR_Default.ts{1}) (qsdgtcr_idx O_MEFGCMA_WOTSTWES.qs{1} R_SMDTTCRC_Game34WOTSTWES.O_R_SMDTTCRC_Game34WOTSTWES.xll{1} ps{1} i0{1} i (j + 1)).
+  nth witness (unzip1 O_SMDTTCR_Default.ts{1}) (qsdgtcr_idx O_MEUFGCMA_WOTSTWES.qs{1} R_SMDTTCRC_Game34WOTSTWES.O_R_SMDTTCRC_Game34WOTSTWES.xll{1} ps{1} i0{1} i (j + 1)).
 + rewrite(nth_map witness witness) //.
   rewrite (: size O_SMDTTCR_Default.ts{1} = size (unzip2 O_SMDTTCR_Default.ts{1})) 1:size_map //. 
   by rewrite rcqsdg qsdgtcridx_rng // neq0_em /#.
 have {1}-> :
-  nth witness (unzip1 O_SMDTTCR_Default.ts{1}) (qsdgtcr_idx O_MEFGCMA_WOTSTWES.qs{1} R_SMDTTCRC_Game34WOTSTWES.O_R_SMDTTCRC_Game34WOTSTWES.xll{1} ps{1} i0{1} i (j + 1))
+  nth witness (unzip1 O_SMDTTCR_Default.ts{1}) (qsdgtcr_idx O_MEUFGCMA_WOTSTWES.qs{1} R_SMDTTCRC_Game34WOTSTWES.O_R_SMDTTCRC_Game34WOTSTWES.xll{1} ps{1} i0{1} i (j + 1))
   = 
-  (set_htbidx (set_chthidx ((nth witness O_MEFGCMA_WOTSTWES.qs{1} i0{1}).`1) i) ((BaseW.val (encode_msgWOTS (nth witness O_MEFGCMA_WOTSTWES.qs{1} i0{1}).`2).[i]) + j)).
+  (set_htbidx (set_chthidx ((nth witness O_MEUFGCMA_WOTSTWES.qs{1} i0{1}).`1) i) ((BaseW.val (encode_msgWOTS (nth witness O_MEUFGCMA_WOTSTWES.qs{1} i0{1}).`2).[i]) + j)).
 + by rewrite rcqsad -eq_qsadtcridx_qsdgtcridx 3:nth_relcqsadtcr_qsadtcridx // neq0_em /= /#.
 have {1}->: 
-  nth witness (unzip1 O_SMDTTCR_Default.ts{1}) (qsdgtcr_idx O_MEFGCMA_WOTSTWES.qs{1} R_SMDTTCRC_Game34WOTSTWES.O_R_SMDTTCRC_Game34WOTSTWES.xll{1} ps{1} i0{1} i (j + 1))
+  nth witness (unzip1 O_SMDTTCR_Default.ts{1}) (qsdgtcr_idx O_MEUFGCMA_WOTSTWES.qs{1} R_SMDTTCRC_Game34WOTSTWES.O_R_SMDTTCRC_Game34WOTSTWES.xll{1} ps{1} i0{1} i (j + 1))
   =
-  (set_htbidx (set_chthidx ((nth witness O_MEFGCMA_WOTSTWES.qs{1} i0{1}).`1) i) ((BaseW.val (encode_msgWOTS m'{1}).[i]) + k)).
+  (set_htbidx (set_chthidx ((nth witness O_MEUFGCMA_WOTSTWES.qs{1} i0{1}).`1) i) ((BaseW.val (encode_msgWOTS m'{1}).[i]) + k)).
 + by rewrite rcqsad -eq_qsadtcridx_qsdgtcridx 3:nth_relcqsadtcr_qsadtcridx // neq0_em /= /#.
 by apply collision_extraction.
 qed.
@@ -6658,38 +6658,38 @@ transitivity Game4_WOTSTWES_Alt.main (={glob A} ==> ={res}) (={glob A} ==> res{1
 proc; inline *.
 swap{2} 13 -11.
 wp => /=.
-seq 9 12 : (   ={glob A, glob O_THFC_Default, O_MEFGCMA_WOTSTWES.qs, ps}
+seq 9 12 : (   ={glob A, glob O_THFC_Default, O_MEUFGCMA_WOTSTWES.qs, ps}
             /\ pp{2} = ps{2}
-            /\ O_MEFGCMA_WOTSTWES.ps{1} = ps{1}
+            /\ O_MEUFGCMA_WOTSTWES.ps{1} = ps{1}
             /\ O_THFC_Default.pp{1} = ps{1}
             /\ O_THFC_Default.pp{2} = ps{2}
             /\ O_SMDTPRE_Default.pp{2} = ps{2}
-            /\ O_MEFGCMA_WOTSTWES.qs{1} = []
-            /\ O_MEFGCMA_WOTSTWES.qs{2} = []
+            /\ O_MEUFGCMA_WOTSTWES.qs{1} = []
+            /\ O_MEUFGCMA_WOTSTWES.qs{2} = []
             /\ O_SMDTPRE_Default.ts{2} = []
             /\ O_THFC_Default.tws{1} = []
             /\ O_THFC_Default.tws{2} = []
             /\ R_SMDTPREC_Game4WOTSTWES.O_R_SMDTPREC_Game4WOTSTWES.adl{2} = []).
 + by auto.
-seq 1 1 : (   ={glob A, O_MEFGCMA_WOTSTWES.qs, ps}
+seq 1 1 : (   ={glob A, O_MEUFGCMA_WOTSTWES.qs, ps}
            /\ pp{2} = ps{2}
-           /\ all (fun (admpksig : adrs * msgWOTS * pkWOTS * sigWOTS) => is_chtype admpksig.`1) O_MEFGCMA_WOTSTWES.qs{1}
-           /\ unzip1 O_SMDTPRE_Default.ts{2} = relcqsad_pre O_MEFGCMA_WOTSTWES.qs{1}
-           /\ unzip2 O_SMDTPRE_Default.ts{2} = relcqsdg_pre O_MEFGCMA_WOTSTWES.qs{1}
+           /\ all (fun (admpksig : adrs * msgWOTS * pkWOTS * sigWOTS) => is_chtype admpksig.`1) O_MEUFGCMA_WOTSTWES.qs{1}
+           /\ unzip1 O_SMDTPRE_Default.ts{2} = relcqsad_pre O_MEUFGCMA_WOTSTWES.qs{1}
+           /\ unzip2 O_SMDTPRE_Default.ts{2} = relcqsdg_pre O_MEUFGCMA_WOTSTWES.qs{1}
            /\ (uniq_preffour (map (fun (admpksig : adrs * msgWOTS * pkWOTS * sigWOTS) => admpksig.`1) 
-                 O_MEFGCMA_WOTSTWES.qs{1})
+                 O_MEUFGCMA_WOTSTWES.qs{1})
                => 
                disj_preffour (map (fun (admpksig : adrs * msgWOTS * pkWOTS * sigWOTS) => admpksig.`1) 
-                 O_MEFGCMA_WOTSTWES.qs{1}) O_THFC_Default.tws{1} 
+                 O_MEUFGCMA_WOTSTWES.qs{1}) O_THFC_Default.tws{1} 
                => 
                disj_lists (unzip1 O_SMDTPRE_Default.ts{2}) O_THFC_Default.tws{2})).
-+ call (:   ={O_MEFGCMA_WOTSTWES.qs, O_THFC_Default.pp}
-         /\ O_MEFGCMA_WOTSTWES.ps{1} = O_SMDTPRE_Default.pp{2}
++ call (:   ={O_MEUFGCMA_WOTSTWES.qs, O_THFC_Default.pp}
+         /\ O_MEUFGCMA_WOTSTWES.ps{1} = O_SMDTPRE_Default.pp{2}
          /\ O_THFC_Default.pp{1} = O_SMDTPRE_Default.pp{2}
-         /\ all (fun (admpksig : adrs * msgWOTS * pkWOTS * sigWOTS) => is_chtype admpksig.`1) O_MEFGCMA_WOTSTWES.qs{1}
-         /\ unzip1 O_SMDTPRE_Default.ts{2} = relcqsad_pre O_MEFGCMA_WOTSTWES.qs{1}
-         /\ unzip2 O_SMDTPRE_Default.ts{2} = relcqsdg_pre O_MEFGCMA_WOTSTWES.qs{1}
-         /\ R_SMDTPREC_Game4WOTSTWES.O_R_SMDTPREC_Game4WOTSTWES.adl{2} = reltqsad_pre O_MEFGCMA_WOTSTWES.qs{1}
+         /\ all (fun (admpksig : adrs * msgWOTS * pkWOTS * sigWOTS) => is_chtype admpksig.`1) O_MEUFGCMA_WOTSTWES.qs{1}
+         /\ unzip1 O_SMDTPRE_Default.ts{2} = relcqsad_pre O_MEUFGCMA_WOTSTWES.qs{1}
+         /\ unzip2 O_SMDTPRE_Default.ts{2} = relcqsdg_pre O_MEUFGCMA_WOTSTWES.qs{1}
+         /\ R_SMDTPREC_Game4WOTSTWES.O_R_SMDTPREC_Game4WOTSTWES.adl{2} = reltqsad_pre O_MEUFGCMA_WOTSTWES.qs{1}
          /\ (forall ad, ad \in O_THFC_Default.tws{2} => 
                ad \in O_THFC_Default.tws{1} \/ ad \in R_SMDTPREC_Game4WOTSTWES.O_R_SMDTPREC_Game4WOTSTWES.adl{2})); last first.
   - skip => /> _ _ _ tws qs ts tws' qsch rcqsad rcqsdg twspmem uqpfqs /hasPn djpfqs.
@@ -6713,7 +6713,7 @@ seq 1 1 : (   ={glob A, O_MEFGCMA_WOTSTWES.qs, ps}
                     let sig_ele = nth witness sig{1} i in
                     nth witness pk{1} i
                     =
-                    cf O_MEFGCMA_WOTSTWES.ps{1} (set_chthidx ad{1} i) 
+                    cf O_MEUFGCMA_WOTSTWES.ps{1} (set_chthidx ad{1} i) 
                       em_ele (w - 1 - em_ele) (val sig_ele)))
              (len - size pk{1}).
     * move=> _ z.
@@ -6726,17 +6726,17 @@ seq 1 1 : (   ={glob A, O_MEFGCMA_WOTSTWES.qs, ps}
            /\ is_chtype ad{2} 
            /\ em{1} = encode_msgWOTS m{1}
            /\ em{2} = encode_msgWOTS m{2}
-           /\ O_MEFGCMA_WOTSTWES.ps{1} = O_SMDTPRE_Default.pp{2}
+           /\ O_MEUFGCMA_WOTSTWES.ps{1} = O_SMDTPRE_Default.pp{2}
            /\ O_THFC_Default.pp{1} = O_SMDTPRE_Default.pp{2}
            /\ unzip1 O_SMDTPRE_Default.ts{2} 
               = 
-              relcqsad_pre O_MEFGCMA_WOTSTWES.qs{1} ++ relcqsad_pre_outer ad{2} m{2} (size pk{2})
+              relcqsad_pre O_MEUFGCMA_WOTSTWES.qs{1} ++ relcqsad_pre_outer ad{2} m{2} (size pk{2})
            /\ unzip2 O_SMDTPRE_Default.ts{2} 
               = 
-              relcqsdg_pre O_MEFGCMA_WOTSTWES.qs{1} ++ relcqsdg_pre_outer m{2} sig{2} (size pk{2})
+              relcqsdg_pre O_MEUFGCMA_WOTSTWES.qs{1} ++ relcqsdg_pre_outer m{2} sig{2} (size pk{2})
            /\ R_SMDTPREC_Game4WOTSTWES.O_R_SMDTPREC_Game4WOTSTWES.adl{2}
               =
-              reltqsad_pre O_MEFGCMA_WOTSTWES.qs{1} ++ reltqsad_pre_outer ad{2} m{2} (size pk{2})
+              reltqsad_pre O_MEUFGCMA_WOTSTWES.qs{1} ++ reltqsad_pre_outer ad{2} m{2} (size pk{2})
            /\ size sig{1} = size pk{2}
            /\ (forall (ad : adrs), ad \in O_THFC_Default.tws{2} =>
                 ad \in O_THFC_Default.tws{1} \/
@@ -6759,7 +6759,7 @@ seq 1 1 : (   ={glob A, O_MEFGCMA_WOTSTWES.qs, ps}
                 /\ em_ele{2} = BaseW.val em{2}.[size pk{2}]
                 /\ R_SMDTPREC_Game4WOTSTWES.O_R_SMDTPREC_Game4WOTSTWES.adl{2}
                    =
-                   reltqsad_pre O_MEFGCMA_WOTSTWES.qs{1} 
+                   reltqsad_pre O_MEUFGCMA_WOTSTWES.qs{1} 
                    ++ reltqsad_pre_outer ad{2} m{2} (size pk{2})
                    ++ reltqsad_pre_inner (set_chthidx ad{2} (size pk{2})) em_ele{2} j{2}
                 /\ size sig{1} = size pk{2}
@@ -6854,7 +6854,7 @@ split => [/# | /lezNgt gelen_szq3 ge1_szqs led_szqs ge0_i0 ltszqs_i0 eqins_pkp n
 split; first by smt(size_map relcqsadpre_rng ge2_len). 
 split; first by rewrite rcqsad uniq_relcqsadpre 1:all_map.
 split => [| /#].
-pose q := nth witness O_MEFGCMA_WOTSTWES.qs{2} i0{2}; rewrite eq_sym in neqq2_mp.
+pose q := nth witness O_MEUFGCMA_WOTSTWES.qs{2} i0{2}; rewrite eq_sym in neqq2_mp.
 move/(nhchwcoll_hchwpre ps{2} q.`1 _ _ q.`4 sig'{2}) /(_ _): (neqq2_mp) => //.
 move=> hchwpre; rewrite eq_sym; pose qsdgidx := qsdgpre_idx _ _ _.
 rewrite -(nth_map witness witness snd qsdgidx O_SMDTPRE_Default.ts{2}).
@@ -6879,8 +6879,8 @@ by apply hchwpre_findprerng.
 qed.
 
 (* Penultimate lemma comprising complete security proof without initial (PRF-reduction) step *)
-lemma MEFGCMA_WOTSTWES_NOPRF &m :
-     Pr[M_EF_GCMA_WOTSTWES(A, O_MEFGCMA_WOTSTWES_NOPRF, O_THFC_Default).main() @ &m : res] 
+lemma MEUFGCMA_WOTSTWES_NOPRF &m :
+     Pr[M_EUF_GCMA_WOTSTWES(A, O_MEUFGCMA_WOTSTWES_NOPRF, O_THFC_Default).main() @ &m : res] 
   <=    (w - 2)%r
         * `|Pr[SM_DT_UD_C(R_SMDTUDC_Game23WOTSTWES(A), O_SMDTUD_Default, O_THFC_Default).main(false) @ &m : res]
             - Pr[SM_DT_UD_C(R_SMDTUDC_Game23WOTSTWES(A), O_SMDTUD_Default, O_THFC_Default).main(true) @ &m : res]| 
@@ -6894,10 +6894,10 @@ have ^ -> ->:
     Pr[SM_DT_UD_C(R_SMDTUDC_DistRCH, O_SMDTUD_Default, O_THFC_Default).main(b) @ &m: res].
 + by move=> b; byequiv=> //; sim.
 have ->:
-  Pr[M_EF_GCMA_WOTSTWES(A, O_MEFGCMA_WOTSTWES_NOPRF, O_THFC_Default).main() @ &m : res]
+  Pr[M_EUF_GCMA_WOTSTWES(A, O_MEUFGCMA_WOTSTWES_NOPRF, O_THFC_Default).main() @ &m : res]
   =
   Pr[Game2_WOTSTWES.main() @ &m : res].
-+ by byequiv MEFGCMA_WOTSTWES_NOPRF_Game2_WOTSTWES. 
++ by byequiv MEUFGCMA_WOTSTWES_NOPRF_Game2_WOTSTWES. 
 have ->:
   Pr[Game2_WOTSTWES.main() @ &m : res]
   =
@@ -6924,8 +6924,8 @@ by apply Step_Game4_WOTSTWES_SMDTPREC.
 qed.
 
 (* Security theorem: Combine previous steps to derive security theorem *)
-lemma MEFGCMA_WOTSTWES &m :
-    Pr[M_EF_GCMA_WOTSTWES(A, O_MEFGCMA_WOTSTWES, O_THFC_Default).main() @ &m : res] 
+lemma MEUFGCMA_WOTSTWES &m :
+    Pr[M_EUF_GCMA_WOTSTWES(A, O_MEUFGCMA_WOTSTWES, O_THFC_Default).main() @ &m : res] 
     <=
   `|Pr[PRF(R_PRF_Game0NOPRFWOTSTWES(A), O_PRF_Default).main(false) @ &m : res] - 
     Pr[PRF(R_PRF_Game0NOPRFWOTSTWES(A), O_PRF_Default).main(true) @ &m : res]|
@@ -6938,26 +6938,26 @@ lemma MEFGCMA_WOTSTWES &m :
     +
     Pr[SM_DT_PRE_C(R_SMDTPREC_Game4WOTSTWES(A), O_SMDTPRE_Default, O_THFC_Default).main() @ &m : res].
 proof.
-move: (MEFGCMA_WOTSTWES_NOPRF &m) => thm_nprf.
+move: (MEUFGCMA_WOTSTWES_NOPRF &m) => thm_nprf.
 have ->:
-  Pr[M_EF_GCMA_WOTSTWES(A, O_MEFGCMA_WOTSTWES, O_THFC_Default).main() @ &m : res] 
+  Pr[M_EUF_GCMA_WOTSTWES(A, O_MEUFGCMA_WOTSTWES, O_THFC_Default).main() @ &m : res] 
   = 
   Pr[Game0_WOTSTWES.main() @ &m : res].
-+ by byequiv MEFGCMA_Game0_WOTSTWES.
++ by byequiv MEUFGCMA_Game0_WOTSTWES.
 have ->:
   Pr[Game0_WOTSTWES.main() @ &m : res]
   =
   `|Pr[Game0_WOTSTWES.main() @ &m : res] - 
-    Pr[M_EF_GCMA_WOTSTWES(A, O_MEFGCMA_WOTSTWES_NOPRF, O_THFC_Default).main() @ &m : res] + 
-    Pr[M_EF_GCMA_WOTSTWES(A, O_MEFGCMA_WOTSTWES_NOPRF, O_THFC_Default).main() @ &m : res]|.
+    Pr[M_EUF_GCMA_WOTSTWES(A, O_MEUFGCMA_WOTSTWES_NOPRF, O_THFC_Default).main() @ &m : res] + 
+    Pr[M_EUF_GCMA_WOTSTWES(A, O_MEUFGCMA_WOTSTWES_NOPRF, O_THFC_Default).main() @ &m : res]|.
 + by smt(ge0_mu).
 apply (ler_trans (  `|Pr[Game0_WOTSTWES.main() @ &m : res] -
-                      Pr[M_EF_GCMA_WOTSTWES(A, O_MEFGCMA_WOTSTWES_NOPRF, O_THFC_Default).main() @ &m : res]|
-                  +   Pr[M_EF_GCMA_WOTSTWES(A, O_MEFGCMA_WOTSTWES_NOPRF, O_THFC_Default).main() @ &m : res])).
-+ rewrite -{4}(ger0_norm Pr[M_EF_GCMA_WOTSTWES(A, O_MEFGCMA_WOTSTWES_NOPRF, O_THFC_Default).main() @ &m : res]). 
+                      Pr[M_EUF_GCMA_WOTSTWES(A, O_MEUFGCMA_WOTSTWES_NOPRF, O_THFC_Default).main() @ &m : res]|
+                  +   Pr[M_EUF_GCMA_WOTSTWES(A, O_MEUFGCMA_WOTSTWES_NOPRF, O_THFC_Default).main() @ &m : res])).
++ rewrite -{4}(ger0_norm Pr[M_EUF_GCMA_WOTSTWES(A, O_MEUFGCMA_WOTSTWES_NOPRF, O_THFC_Default).main() @ &m : res]). 
   - by rewrite Pr[mu_ge0]. 
   by apply ler_norm_add.
-by rewrite -2!addrA ler_add 1:Step_Game0_MEFGCMA_WOTSTWES_NOPRF_PRF // addrA.
+by rewrite -2!addrA ler_add 1:Step_Game0_MEUFGCMA_WOTSTWES_NOPRF_PRF // addrA.
 qed.
 
-end section Proof_M_EF_GCMA_WOTSTWES.
+end section Proof_M_EUF_GCMA_WOTSTWES.
